core/theories/Core/Impure.v
@@ -18,578 +18,43 @@
  * along with this program. If not, see <http://www.gnu.org/licenses/>.
  *)
 
-(** In this library, we provide all the necessary concepts to model interacting
-    components using Coq.  We do that by means of a variant of the Free monad
-    introduced by the Haskell <<operational>> package, and originally called the
-    Program monad thereafter.  The Program monad is parameterized by a type
-    which describes the interfaces its monadic computations can use, where an
-    interface describes a set of functions carried out by an outer environment
-    expected to produce a result.  In other words, using the <<operational>>
-    Program monad, we model impurity.
+(** In [FreeSpec.Core.Interface], we have introduced the [interface] type, to
+    model the set of primitives an impure computation can use. We also introduce
+    [MayProvide], [Provide] and [Distinguish]. They are three type classes which
+    allow for manipulating _polymorphic interface composite_.
 
-    To avoid ambiguity with the Program framework of Coq, we rename the Program
-    monad the [impure] monad, and we call “impure computations” the monadic
-    computations which happens within the [impure] monad.  We call “primitives”
-    the impure functions provided by a given interface.
 
-    The key idea behind FreeSpec is to model components as functions which maps
-    primitives of the interface it exposes to impure computations parameterized
-    by the interfaces it uses. *)
+    In this library, we provide the [impure] monad, defined after the
+    <<Program>> monad introduced by the <<operational>> package (see
+    <<https://github.com/whitequark/unfork#introduction>>). *)
 
-From Coq.Program Require Import Equality Tactics Basics.
-From Coq Require Import Morphisms.
-From Coq Require Import Relations Setoid Morphisms.
-From Prelude Require Import Equality Control Control.Classes Tactics State.
-
-#[local]
-Open Scope monad_scope.
+From Coq Require Import Program Setoid Morphisms.
+From Prelude Require Import All.
+From FreeSpec.Core Require Import Interface.
 
 #[local]
 Open Scope signature_scope.
 
-#[local]
-Open Scope prelude_scope.
-
-Notation "''equal'" := (@equal _ _) (only parsing).
-
-(** * Interfaces *)
-
-(** Following the definition of the <<operational>> package, interfaces in
-    FreeSpec are parameterized inductive types whose terms purposely describe
-    the primitives the interface provides. *)
-
-Definition interface := Type -> Type.
-
-(** Given [i : interface], a term of type [i α] identifies a primitive of [i]
-    expected to produce a result of type [α].
-
-    The simpler interface is the empty interface, which provides no primitives
-    whatsoever. *)
-
-Inductive iempty : interface := .
-Notation "'<>'" := iempty : type_scope.
-Notation "'⋄'" := iempty : type_scope.
-
-(** To use the [⋄] interface to parameterize the [impure] monad is equivalent to
-    writing pure functions.
-
-    Another example of general-purpose interface we can define is the [STORE s]
-    interface, where [s] is a type, and [STORE s] allows for manipulating a
-    global, mutable variable of type [s] within an impure computation. *)
-
-Inductive STORE (s : Type) : interface :=
-| Get : STORE s s
-| Put (x : s) : STORE s unit.
-
-Arguments Get {s}.
-Arguments Put [s] (x).
-
-(** According to the definition of [STORE s], an impure computation can use two
-    primitives. The term [Get : STORE s s] describes a primitive expected to
-    produce a result of type [s], that is the current value of the mutable
-    variable.  Terms of the form [Put x : STORE s unit] describe a primitive
-    which does not produce any meaningful result, but is expected to update the
-    current value of the mutable variable.
-
-    The use of the word “expected” to describe the primitive of [STORE s] is
-    voluntary.  The definition of a semantics does not attach any particular
-    semantics to the primitives it describes.  This will come latter, and in
-    fact, one interface may have many legitimate semantics.
-
-    Impure computations are likely to use more than one interface, but the
-    [impure] monad takes only one argument.  We introduce [iplus] (denoted by
-    [<+>] or [⊕]) to compose interfaces together.  An impure computation
-    parameterized by [i ⊕ j] can therefore leverages the privimites of both [i]
-    and [j]. *)
-
-Inductive iplus (i j : interface) (a : Type) :=
-| in_left (e : i a) : iplus i j a
-| in_right (e : j a) : iplus i j a.
-
-Arguments in_left [i j a] (e).
-Arguments in_right [i j a] (e).
-
-Register iplus as freespec.core.iplus.type.
-Register in_left as freespec.core.iplus.in_left.
-Register in_right as freespec.core.iplus.in_right.
-
-Infix "<+>" := iplus (at level 50, left associativity) : type_scope.
-Infix "⊕" := iplus (at level 50, left associativity) : type_scope.
-
-(** When defining general-purpose impure computations that we expect to reuse in
-    different context, we want to leave the interface as a parameter, and rather
-    express the constrains in terms of interface availability.  To do that, we
-    introduce the [Provide] typeclass, such that [Provide ix i] implies impure
-    computations parameterized by [ix] can use primitives of [i]. *)
-
-Class MayProvide (ix i : interface) : Type :=
-  { unlift_eff {a : Type} (e : ix a) : option (i a)
-  }.
-
-(* WARNING: [Provide] takes a [MayProvide] instance as argument rather than
-   embedding one for good reasons, and one shall be fully aware of this fact
-   before attempting (and failing) to change it. *)
-
-Class Provide (ix i : interface) `{MayProvide ix i} : Type :=
-  { lift_eff {a : Type} (e : i a) : ix a
-  ; unlift_lift_equ {a : Type} (e : i a) : unlift_eff (lift_eff e) = Some e
-  }.
-
-Instance default_MayProvide (i j : interface) : MayProvide i j|1000 :=
-  { unlift_eff := fun _ _ => None
-  }.
-
-Instance refl_MayProvide (i : interface) : MayProvide i i :=
-  { unlift_eff := fun (a : Type) (e : i a) => Some e
-  }.
-
-#[program]
-Instance refl_Provide (i : interface) : Provide i i :=
-  { lift_eff := fun (a : Type) (e : i a) => e
-  }.
-
-Instance iplus_left_MayProvide (ix i j : interface) `{MayProvide ix i}
-  : MayProvide (ix ⊕ j) i :=
-  { unlift_eff := fun (a : Type) (e : (ix ⊕ j) a) =>
-                    match e with
-                    | in_left e => unlift_eff e
-                    | _ => None
-                    end
-  }.
-
-#[program]
-Instance iplus_left_Provide (ix i j : interface)
-   `{H : MayProvide ix i} `{@Provide ix i H}
-  : @Provide (ix ⊕ j) i (iplus_left_MayProvide ix i j) :=
-  { lift_eff := fun (a : Type) (e : i a) => in_left (lift_eff e)
-  }.
-
-Next Obligation.
-  now rewrite unlift_lift_equ.
-Qed.
-
-Instance iplus_right_MayProvide (i jx j : interface) `{MayProvide jx j}
-  : MayProvide (i ⊕ jx) j :=
-  { unlift_eff := fun (a : Type) (e : (i ⊕ jx) a) =>
-                    match e with
-                    | in_right e => unlift_eff e
-                    | _ => None
-                    end
-  }.
-
-#[program]
-Instance iplus_right_Provide (i jx j : interface)
-   `{H : MayProvide jx j} `{@Provide jx j H}
-  : @Provide (i ⊕ jx) j (iplus_right_MayProvide i jx j) :=
-  { lift_eff := fun (a : Type) (e : j a) => in_right (lift_eff e)
-  }.
-
-Next Obligation.
-  now rewrite unlift_lift_equ.
-Qed.
-
-Ltac find_may_provide :=
-  apply refl_MayProvide + (eapply iplus_left_MayProvide; find_may_provide) + (eapply iplus_right_MayProvide; find_may_provide).
-
-Hint Extern 1 (MayProvide (iplus _ _) _) => find_may_provide : typeclass_instances.
-
-Class Distinguish (ix i j : interface) `{Provide ix i} `{MayProvide ix j} : Prop :=
-  { distinguish : forall {a} (e : i a), unlift_eff (i := j) (lift_eff (ix := ix) e) = None
-  }.
-
-#[program]
-Instance refl_Distinguish (i j : interface)
-  : @Distinguish i i j  (@refl_MayProvide i) (@refl_Provide i) (@default_MayProvide i j).
-
-#[program]
-Instance iplus_left_default_Distinguish (ix jx i j : interface)
-   `{M1 : MayProvide ix i} `{P1 : @Provide ix i M1}
-  : @Distinguish (ix ⊕ jx) i j
-                 (@iplus_left_MayProvide ix i jx M1)
-                 (@iplus_left_Provide ix i jx M1 P1)
-                 (@default_MayProvide _ j).
-
-#[program]
-Instance iplus_right_default_Distinguish (ix jx i j : interface)
-   `{M1 : MayProvide jx i} `{P1 : @Provide jx i M1}
-  : @Distinguish (ix ⊕ jx) i j
-                 (@iplus_right_MayProvide ix jx i M1)
-                 (@iplus_right_Provide ix jx i M1 P1)
-                 (@default_MayProvide _ j).
-
-#[program]
-Instance iplus_left_may_right_Distinguish (ix jx i j : interface)
-   `{M1 : MayProvide ix i} `{P1 : @Provide ix i M1} `{M2 : MayProvide jx j}
-  : @Distinguish (ix ⊕ jx) i j
-                 (@iplus_left_MayProvide ix i jx M1)
-                 (@iplus_left_Provide ix i jx M1 P1)
-                 (@iplus_right_MayProvide ix jx j M2).
-
-#[program]
-Instance iplus_right_may_left_Distinguish (ix jx i j : interface)
-   `{M1 : MayProvide jx i} `{P1 : @Provide jx i M1} `{M2 : MayProvide ix j}
-  : @Distinguish (ix ⊕ jx) i j
-                 (@iplus_right_MayProvide ix jx i M1)
-                 (@iplus_right_Provide ix jx i M1 P1)
-                 (@iplus_left_MayProvide ix j jx M2).
-
-#[program]
-Instance iplus_left_distinguish_left_Distinguish (ix jx i j : interface)
-   `{M1 : MayProvide ix i} `{P1 : @Provide ix i M1} `{M2 : MayProvide ix j}
-   `{@Distinguish ix i j M1 P1 M2}
-  : @Distinguish (ix ⊕ jx) i j
-                 (@iplus_left_MayProvide ix i jx M1)
-                 (@iplus_left_Provide ix i jx M1 P1)
-                 (@iplus_left_MayProvide ix j jx M2).
-
-Next Obligation.
-  apply distinguish.
-Defined.
-
-#[program]
-Instance iplus_right_distinguish_right_Distinguish (ix jx i j : interface)
-   `{M1 : MayProvide jx i} `{P1 : @Provide jx i M1} `{M2 : MayProvide jx j}
-   `{@Distinguish jx i j M1 P1 M2}
-  : @Distinguish (ix ⊕ jx) i j
-                 (@iplus_right_MayProvide ix jx i M1)
-                 (@iplus_right_Provide ix jx i M1 P1)
-                 (@iplus_right_MayProvide ix jx j M2).
-
-Next Obligation.
-  apply distinguish.
-Defined.
-
-(** We introduce a dedicated notation for conveniently declare interface
-    requirements.  Our main source of inspiration is the PureScript row of
-    effects.
-
-    Afterwards, we can write [`{ix :| INTERFACE1, INTERFACE2}] to say that [ix]
-    provides at least [INTERFACE1] and [INTERFACE2] primitives. *)
-
-(** * Operational Semantics *)
-
-(** We have already explained interfaces, in FreeSpec, does not attach any
-    particular semantics to their primitives.  Once an interface has been
-    defined, we can provide one (or more) operational semantics to interpret its
-    primitives. *)
-
-(** ** Definition *)
-
-(** An operational [semantics] for the interface [i] is coinductively defined as
-    a function which can be used to interpret any primitive of [i]; it produces
-    an [interp_out] terms. *)
-
-CoInductive semantics (i : interface) : Type :=
-| mk_semantics (f : forall (a : Type), i a -> interp_out i a) : semantics i
-
-(** A term of type [interp_out i a] is therefore the result of the
-    interpretation of a given primitive [i a]. It provides a result for this
-    primitive (of type [a]), and the new semantics to use to interpret the next
-    primitive of [i]. *)
-
-with interp_out (i : interface) : Type -> Type :=
-| mk_out {a} (x : a) (sem : semantics i) : interp_out i a.
-
-Arguments mk_semantics [i] (f).
-Arguments mk_out [i a] (x sem).
-
-(** Thus, a [semantics] does not only compute a result for a primitive, but also
-    provides a new semantics.  This is necessary to model impurity: the same
-    primitive may or may not return the same result when called several
-    times. *)
-
-(** As for interfaces, the simpler [semantics] is the operational semantics for
-    [⋄], the empty interface. *)
-
-Definition semempty : semantics ⋄ :=
-  mk_semantics (fun (a : Type) (e : iempty a) => match e with end).
-
-(** As an example, we provide a semantics for the [STORE s] interface: *)
-
-CoFixpoint store {s} (init : s) : semantics (STORE s) :=
-  mk_semantics (fun (a : Type) (e : STORE s a) =>
-                  match e with
-                  | Get => mk_out init (store init)
-                  | Put next => mk_out tt (store next)
-                  end).
-
-(** We provide several helper functions to interpret primitives with
-    semantics. *)
-
-Definition run_effect {i a} (sem : semantics i) (e : i a) : interp_out i a :=
-  match sem with mk_semantics f => f _ e end.
-
-Definition interp_result {i a} (step : interp_out i a) : a :=
-  match step with mk_out x _ => x end.
-
-Definition interp_next {i a} (step : interp_out i a) : semantics i :=
-  match step with mk_out _ sem => sem end.
-
-Definition eval_effect {i a} (sem : semantics i) (e : i a) : a :=
-  interp_result (run_effect sem e).
-
-Definition exec_effect {i a} (sem : semantics i) (e : i a) : semantics i :=
-  interp_next (run_effect sem e).
-
-(** Besides, and similarly to interfaces, operational semantics can and should
-    be composed together.  To that end, we provide the [semplus] operation
-    (denoted by [<+>] or [⊕]). *)
-
-CoFixpoint semplus {i j} (sem_i : semantics i) (sem_j : semantics j)
-  : semantics (i ⊕ j) :=
-  mk_semantics (fun (a : Type) (e : (i ⊕ j) a) =>
-                  match e with
-                  | in_left e =>
-                    let out := run_effect sem_i e in
-                    mk_out (interp_result out) (semplus (interp_next out) sem_j)
-                  | in_right e =>
-                    let out := run_effect sem_j e in
-                    mk_out (interp_result out) (semplus sem_i (interp_next out))
-                  end).
-
-Declare Scope semantics_scope.
-
-Infix "<x>" := semplus (at level 50, left associativity) : semantics_scope.
-Infix "⊗" := semplus (at level 50, left associativity) : semantics_scope.
-
-Bind Scope semantics_scope with semantics.
-
-(** ** Equivalence *)
-
-(** We say two semantics are equivalent when (1) we they produce equivalent
-    outputs given the same primitive. *)
-
-CoInductive semantics_equiv {i} : semantics i -> semantics i -> Prop :=
-| semantics_equiv_rec
-    (sem sem' : semantics i)
-    (step_equiv : forall {a} (e : i a),
-        interp_out_equiv (run_effect sem e) (run_effect sem' e))       (* (1) *)
-  : semantics_equiv sem sem'
-
-(** Two interpretation output are said equivalent when (1) they carry the same
-    result, and they provide equivalent semantics to use afterwards. *)
-
-with interp_out_equiv {i} : forall {a : Type}, interp_out i a -> interp_out i a -> Prop :=
-| step_equiv {a}
-    (o o' : interp_out i a)
-    (res_eq : interp_result o = interp_result o')                      (* (1) *)
-    (next_equiv : semantics_equiv (interp_next o) (interp_next o'))    (* (2) *)
-  : interp_out_equiv o o'.
-
-(** We prove [semantics_equiv] is an equivalence, that is the relation is (1)
-    reflexive, (2) symmetric, and (3) transitive. *)
-
-#[program]
-Instance semantics_equiv_Equivalence (i : interface) : Equivalence (@semantics_equiv i).
-
-Obligation 1.
-  cofix semantics_equiv_refl.
-  intros sem.
-  constructor.
-  intros a e.
-  constructor; [ reflexivity |].
-  apply semantics_equiv_refl.
-Qed.
-
-Obligation 2.
-  cofix semantics_equiv_sym.
-  intros sem sem' equiv.
-  destruct equiv as [sem sem' step].
-  constructor.
-  intros a e.
-  specialize step with a e.
-  destruct step.
-  constructor.
-  + now symmetry.
-  + now apply semantics_equiv_sym.
-Qed.
-
-Obligation 3.
-  cofix semantics_equiv_trans.
-  intros sem sem' sem'' equiv equiv'.
-  destruct equiv as [sem sem' equ].
-  destruct equiv' as [sem' sem'' equ'].
-  constructor; intros a e.
-  specialize equ with a e.
-  specialize equ' with a e.
-  inversion equ; ssubst.
-  inversion equ'; ssubst.
-  constructor.
-  + now transitivity (eval_effect sem' e).
-  + eapply semantics_equiv_trans; [ apply next_equiv | apply next_equiv0 ].
-Qed.
-
-(** We use [semantics_equiv] as the [Equality] relation for [semantics]. *)
-
-#[program]
-Instance semantics_Equality (i : interface) : Equality (semantics i).
-
-#[global]
-Opaque semantics_Equality.
-
-(** We proceed similarly with [interp_out_equiv]: we first prove it is an
-    equivalence, then we use this relation as the [Equality] relation for
-    [interp_out]. *)
-
-#[program]
-Instance interp_out_Equivalence (i : interface) (a : Type)
-  : Equivalence (@interp_out_equiv i a).
-
-Obligation 1.
-  intros [x sem].
-  constructor; reflexivity.
-Qed.
-
-Obligation 2.
-  intros o o' equ.
-  inversion equ; ssubst.
-  now constructor.
-Qed.
-
-Obligation 3.
-  intros o o' o'' equ equ'.
-  inversion equ; ssubst.
-  inversion equ'; ssubst.
-  constructor.
-  + now transitivity (interp_result o').
-  + now transitivity (interp_next o').
-Qed.
-
-#[program]
-Instance interp_out_Equality (i : interface) (a : Type) : Equality (interp_out i a).
-
-#[global]
-Opaque interp_out_Equality.
-
-(** Since [interp_out_equiv] and [semantics_equiv] are two equivalence, we can
-    use them with the [rewrite] tactics, as long as we provide valid [Proper]
-    instances.  We proceed accordingly in FreeSpec.Core, as systematically as
-    possible. *)
-
-#[program]
-Instance mk_out_Proper (i : interface) (a : Type)
-  : Proper (eq ==> 'equal ==> 'equal) (@mk_out i a).
-
-Next Obligation.
-  add_morphism_tactic.
-  intros x sem sem' equ.
-  constructor.
-  + reflexivity.
-  + apply equ.
-Qed.
-
-#[program]
-Instance run_effect_Proper (i : interface) (a : Type)
-  : Proper ('equal ==> eq ==> 'equal) (@run_effect i a).
-
-Next Obligation.
-  add_morphism_tactic.
-  intros sem sem' equ p.
-  inversion equ; ssubst.
-  apply step_equiv0.
-Qed.
-
-#[program]
-Instance interp_result_Proper (i : interface) (a : Type)
-  : Proper ('equal ==> eq) (@interp_result i a).
-
-Next Obligation.
-  add_morphism_tactic.
-  intros o o' equ.
-  now inversion equ; ssubst.
-Qed.
-
-#[program]
-Instance interp_next_Proper (i : interface) (a : Type)
-  : Proper ('equal ==> 'equal) (@interp_next i a).
-
-Next Obligation.
-  add_morphism_tactic.
-  intros o o' equ.
-  now inversion equ; ssubst.
-Qed.
-
-#[program]
-Instance eval_effect_Proper (i : interface) (a : Type)
-  : Proper ('equal ==> eq ==> eq) (@eval_effect i a).
-
-Next Obligation.
-  add_morphism_tactic.
-  intros o o' equ e.
-  unfold eval_effect.
-  now rewrite equ.
-Qed.
-
-#[program]
-Instance exec_effect_Proper (i : interface) (a : Type)
-  : Proper ('equal ==> eq ==> 'equal) (@exec_effect i a).
-
-Next Obligation.
-  add_morphism_tactic.
-  intros o o' equ e.
-  unfold exec_effect.
-  now rewrite equ.
-Qed.
-
-Lemma semantics_equiv_interp_next_effect {i a}
-  (sem sem' : semantics i) (equ : sem == sem') (e : i a)
-  : interp_next (run_effect sem e) == interp_next (run_effect sem' e).
-Proof.
-  inversion equ; ssubst.
-  specialize step_equiv0 with a e.
-  inversion step_equiv0; ssubst.
-  apply next_equiv.
-Qed.
-
-Hint Resolve semantics_equiv_interp_next_effect : freespec.
-
-Lemma semantics_equiv_exec_effect {i a}
-  (sem sem' : semantics i) (equ : sem == sem') (e : i a)
-  : exec_effect sem e == exec_effect sem' e.
-Proof.
-  unfold exec_effect.
-  auto with freespec.
-Qed.
-
-Hint Resolve semantics_equiv_exec_effect : freespec.
-
-#[program]
-Instance semplus_Proper (i j : interface)
-  : Proper ('equal ==> 'equal ==> 'equal) (@semplus i j).
-
-Next Obligation.
-  add_morphism_tactic.
-  cofix semplus_Proper.
-  intros semi semi' equi semj semj' equj.
-  constructor.
-  intros a e.
-  destruct e; constructor; cbn.
-  + now rewrite equi.
-  + apply semplus_Proper; auto with freespec.
-  + now rewrite equj.
-  + apply semplus_Proper; auto with freespec.
-Qed.
-
 (** * Impure Computations *)
 
 (** We introduce the [impure] monad to describe impure computations, that is
-    computations which uses primitives from certain interfaces.
+    computations which uses primitives from certain interfaces. *)
 
-    ** Definition
+(** ** Definition *)
 
-    The [impure] monad is an inductive datatype with two parameters: the
-    interface [i] to be used, and the type [a] of the result of the computation.
+(** The [impure] monad is an inductive datatype with two parameters: the
+    interface [i] to be used, and the type [α] of the result of the computation.
     The fact that [impure] is inductive rather than co-inductive means it is not
-    possible to describte infinite computations.  This also means it is possible
+    possible to describe infinite computations.  This also means it is possible
     to interpret impure computation within Coq, providing an operational
     semantics for [i]. *)
 
-Inductive impure (i : interface) (a : Type) : Type :=
-| local (x : a) : impure i a
-| request_then {b} (e : i b) (f : b -> impure i a) : impure i a.
+Inductive impure (i : interface) (α : Type) : Type :=
+| local (x : α) : impure i α
+| request_then {β} (e : i β) (f : β -> impure i α) : impure i α.
 
-Arguments local [i a] (x).
-Arguments request_then [i a b] (e f).
+Arguments local [i α] (x).
+Arguments request_then [i α β] (e f).
 
 Register impure as freespec.core.impure.type.
 Register local as freespec.core.impure.local.
@@ -605,12 +70,12 @@ Register request_then as freespec.core.impure.request_then.
 
     The definition of [impure_equiv] is two-fold. *)
 
-Inductive impure_equiv {i a} : impure i a -> impure i a -> Prop  :=
+Inductive impure_equiv {i α} : impure i α -> impure i α -> Prop  :=
 
 (** - Two impure computations are equivalent if and only if they compute the
       exact same term (wrt. Coq [eq] function). *)
 
-| local_equiv (x : a) : impure_equiv (local x) (local x)
+| local_equiv (x : α) : impure_equiv (local x) (local x)
 
 (** - Two computations which consist in requesting the interpretation of an
       primitive and passing the result to a monadic continuation are equivalent
@@ -618,8 +83,8 @@ Inductive impure_equiv {i a} : impure i a -> impure i a -> Prop  :=
       given any result the interpretation of this primitive may produce, their
       continuation returns equivalent impure computations. *)
 
-| request_equiv {b} (e : i b) (f g : b -> impure i a)
-    (equ : forall (x : b), impure_equiv (f x) (g x))
+| request_equiv {β} (e : i β) (f g : β -> impure i α)
+    (equ : forall (x : β), impure_equiv (f x) (g x))
   : impure_equiv (request_then e f) (request_then e g).
 
 (** The definition of [impure_equiv] is very similar to [eq], with the exception
@@ -627,8 +92,7 @@ Inductive impure_equiv {i a} : impure i a -> impure i a -> Prop  :=
     proving this is indeed a proper equivalence. *)
 
 #[program]
-Instance impure_equiv_Equivalence (i : interface) (a : Type)
-  : Equivalence (@impure_equiv i a).
+Instance impure_equiv_Equivalence : Equivalence (@impure_equiv i α).
 
 Next Obligation.
   intros p.
@@ -653,11 +117,11 @@ Next Obligation.
   + inversion pq; ssubst; inversion qr; ssubst.
     constructor.
     intros x.
-    now apply H with (b := x).
+    now apply H with (β := x).
 Qed.
 
 #[program]
-Instance impure_Equality (i : interface) (a : Type) : Equality (impure i a).
+Instance impure_Equality : Equality (impure i α).
 
 #[global]
 Opaque impure_Equality.
@@ -668,8 +132,7 @@ Opaque impure_Equality.
    Equality for [a -> b] is [forall x, f x = g x], which is exactly what we
    need. *)
 #[program]
-Instance request_then_Proper (i : interface) (a b : Type)
-  : Proper (eq ==> 'equal ==> 'equal) (@request_then i a b).
+Instance request_then_Proper : Proper (eq ==> 'equal ==> 'equal) (@request_then i α β).
 
 Next Obligation.
   add_morphism_tactic.
@@ -682,15 +145,14 @@ Qed.
 (** We then provide the necessary instances of the <<coq-prelude>> Monad
     typeclasses hierarchy. *)
 
-Fixpoint impure_bind {i a b} (p : impure i a) (f : a -> impure i b) : impure i b :=
+Fixpoint impure_bind {i α β} (p : impure i α) (f : α -> impure i β) : impure i β :=
   match p with
   | local x => f x
   | request_then e g => request_then e (fun x => impure_bind (g x) f)
   end.
 
 #[program]
-Instance impure_bind_Proper_1 (i : interface) (a b : Type)
-  : Proper (eq ==> 'equal ==> 'equal) (@impure_bind i a b).
+Instance impure_bind_Proper_1 : Proper (eq ==> 'equal ==> 'equal) (@impure_bind i α β).
 
 Next Obligation.
   add_morphism_tactic.
@@ -703,8 +165,7 @@ Next Obligation.
 Qed.
 
 #[program]
-Instance impure_bind_Proper_2 (i : interface) (a b : Type)
-  : Proper ('equal ==> eq ==> 'equal) (@impure_bind i a b).
+Instance impure_bind_Proper_2 : Proper ('equal ==> eq ==> 'equal) (@impure_bind i α β).
 
 Next Obligation.
   add_morphism_tactic.
@@ -730,7 +191,8 @@ Ltac change_impure_bind :=
     assert (R: f == g); [ intros ?x | now rewrite R ]
   end.
 
-Lemma impure_bind_local {i a} (p : impure i a) : impure_bind p (@local i a) == p.
+Lemma impure_bind_local {i α} (p : impure i α) : impure_bind p (fun x => local x) == p.
+
 Proof.
   induction p.
   + reflexivity.
@@ -739,9 +201,10 @@ Proof.
     now rewrite H.
 Qed.
 
-Lemma impure_bind_assoc {i a b c}
-  (p : impure i a) (f : a -> impure i b) (g : b -> impure i c)
+Lemma impure_bind_assoc {i α β δ}
+  (p : impure i α) (f : α -> impure i β) (g : β -> impure i δ)
   : impure_bind (impure_bind p f) g == impure_bind p (fun x => impure_bind (f x) g).
+
 Proof.
   induction p; [reflexivity |].
   cbn.
@@ -750,12 +213,11 @@ Proof.
 Qed.
 
 (* see FIXME[0] *)
-Definition impure_map {i a b} (f : a -> b) (p : impure i a) : impure i b :=
+Definition impure_map {i α β} (f : α -> β) (p : impure i α) : impure i β :=
   impure_bind p (fun x => local (f x)).
 
 #[program]
-Instance impure_map_Proper (i : interface) (a b : Type)
-  : Proper ('equal ==> 'equal ==> 'equal) (@impure_map i a b).
+Instance impure_map_Proper : Proper ('equal ==> 'equal ==> 'equal) (@impure_map i α β).
 
 Next Obligation.
   add_morphism_tactic.
@@ -767,7 +229,7 @@ Next Obligation.
 Qed.
 
 #[program]
-Instance impure_Functor (i : interface) : Functor (impure i) :=
+Instance impure_Functor : Functor (impure i) :=
   { map := @impure_map i
   }.
 
@@ -782,15 +244,13 @@ Next Obligation.
   now rewrite impure_bind_assoc.
 Defined.
 
-Definition impure_pure {i a} : a -> impure i a :=
-  @local i a.
+Definition impure_pure {i α} (x : α) : impure i α := local x.
 
-Definition impure_apply {i a b} (p : impure i (a -> b)) (q : impure i a) : impure i b :=
+Definition impure_apply {i α β} (p : impure i (α -> β)) (q : impure i α) : impure i β :=
   impure_bind p (fun f => map f q).
 
 #[program]
-Instance impure_apply_Proper (i : interface) (a b : Type)
-  : Proper ('equal ==> 'equal ==> 'equal) (@impure_apply i a b).
+Instance impure_apply_Proper : Proper ('equal ==> 'equal ==> 'equal) (@impure_apply i α β).
 
 Next Obligation.
   add_morphism_tactic.
@@ -803,7 +263,7 @@ Next Obligation.
 Qed.
 
 #[program, universes(polymorphic)]
-Instance impure_Applicative (i : interface) : Applicative (impure i) :=
+Instance impure_Applicative : Applicative (impure i) :=
   { pure := @impure_pure i
   ; apply := @impure_apply i
   }.
@@ -869,15 +329,15 @@ Defined.
     function from the [Monad] typeclass allows for seamlessly combine impure
     computations together.
 
-    To complete these two monadic operation, we introduce the [request]
+    To complete these two monadic operations, we introduce the [request]
     function, whose purpose is to define an impure computation that uses a given
     primitive [e] from an interface [i], and returns its result.  [request] does
     not parameterize the [impure] monad with [i] directly, but rather with a
     generic interface [ix].  [ix] is constrained with the [Provide] notation, so
     that it has to provide at least [i]'s primitives.  *)
 
-Definition request {ix i} `{Provide ix i} {a : Type} (e : i a) : impure ix a :=
-  request_then (lift_eff e) (fun x => local x).
+Definition request `{Provide ix i} {α} (e : i α) : impure ix α :=
+  request_then (inj_p e) (fun* x => pure x).
 
 (** Note: there have been attempts to turn [request] into a typeclass
     function (to seamlessly use [request] with a [MonadTrans] instance such as
@@ -889,8 +349,9 @@ Definition request {ix i} `{Provide ix i} {a : Type} (e : i a) : impure ix a :=
 
     The <<coq-prelude>> provides notations (inspired by the do notation of
     Haskell) to write monadic functions more easily.  These notations live
-    inside the [monad_scope] scope. *)
+    inside the [monad_scope]. *)
 
+Declare Scope impure_scope.
 Bind Scope monad_scope with impure.
 
 Instance store_monad_state (s : Type) (ix : interface) `{Provide ix (STORE s)}
@@ -898,225 +359,3 @@ Instance store_monad_state (s : Type) (ix : interface) `{Provide ix (STORE s)}
   { put := fun (x : s) => request (Put x)
   ; get := request Get
   }.
-
-(** ** Interpreting Impure Computations *)
-
-(** A term of type [impure a] describes an impure computation expected to return
-    a term of type [a].  Interpreting this term means actually realizing the
-    computation and producing the result.  This requires to provide an
-    operational semantics for the interfaces used by the computation.
-
-    Some operational semantics may be defined in Gallina by means of the
-    [semantics] type. In such a case, we provide helpers functions to use them
-    in conjunction with [impure] terms. The terminology follows a similar logic than the
-    Haskell state monad:
-
-    - [run_impure] interprets an impure computation [p] with an operational
-      semantics [sem], and returns both the result of [p] and the new
-      operational semantics to use afterwards.
-    - [eval_impure] only returns the result of [p].
-    - [exec_impure] only returns the new operational semantics. *)
-
-Fixpoint run_impure {i a} (sem : semantics i) (p : impure i a) : interp_out i a :=
-  match p with
-  | local x =>
-    mk_out x sem
-  | request_then e f =>
-    let s := run_effect sem e in
-    run_impure (interp_next s) (f (interp_result s))
-  end.
-
-Definition eval_impure {i a} (sem : semantics i) (p : impure i a) : a :=
-  interp_result (run_impure sem p).
-
-Definition exec_impure {i a} (sem : semantics i) (p : impure i a) : semantics i :=
-  interp_next (run_impure sem p).
-
-(** We provide several lemmas and the necessary [Proper] instances to use these
-    functions in conjunction with [semantics_equiv] and [impure_equiv]. *)
-
-Lemma run_impure_request_then_equ {i a b} (sem : semantics i)
-  (e : i a) (f : a -> impure i b)
-  : run_impure sem (request_then e f) = run_impure (exec_effect sem e) (f (eval_effect sem e)).
-Proof eq_refl.
-
-Hint Rewrite @run_impure_request_then_equ : freespec.
-
-Lemma semantics_equiv_interp_next_impure {i a}
-  (sem sem' : semantics i) (equ : sem == sem') (p : impure i a)
-  : interp_next (run_impure sem p) == interp_next (run_impure sem' p).
-Proof.
-  revert sem sem' equ.
-  induction p; intros sem sem' equ.
-  + apply equ.
-  + cbn.
-    unfold exec_impure.
-    cbn.
-    rewrite equ at 2.
-    apply H.
-    auto with freespec.
-Qed.
-
-Hint Resolve semantics_equiv_interp_next_impure : freespec.
-
-Lemma semantics_equiv_exec_impure {i a}
-  (sem sem' : semantics i) (equ : sem == sem') (p : impure i a)
-  : exec_impure sem p == exec_impure sem' p.
-Proof.
-  unfold exec_impure.
-  auto with freespec.
-Qed.
-
-Hint Resolve semantics_equiv_exec_impure : freespec.
-
-#[program]
-Instance run_impure_Proper_1 (i : interface) (a : Type)
-  : Proper ('equal ==> eq ==> 'equal) (@run_impure i a).
-
-Next Obligation.
-  add_morphism_tactic.
-  intros sem sem' equ p.
-  revert sem sem' equ.
-  induction p; intros sem sem' equ.
-  + cbn.
-    now rewrite equ.
-  + cbn.
-    rewrite equ at 2.
-    auto with freespec.
-Qed.
-
-#[program]
-Instance run_impure_Proper_2 (i : interface) (a : Type)
-  : Proper (eq ==> 'equal ==> 'equal) (@run_impure i a).
-
-Next Obligation.
-  add_morphism_tactic.
-  intros sem p q equ.
-  revert sem.
-  induction equ; intros sem.
-  + reflexivity.
-  + apply H.
-Qed.
-
-#[program]
-Instance eval_impure_Proper (i : interface) (a : Type)
-  : Proper ('equal ==> 'equal ==> eq) (@eval_impure i a).
-
-Next Obligation.
-  add_morphism_tactic.
-  intros sem sem' equ1 p q equ2.
-  unfold eval_impure.
-  now rewrite equ1, equ2.
-Qed.
-
-#[program]
-Instance exec_impure_Proper (i : interface) (a : Type)
-  : Proper ('equal ==> 'equal ==> 'equal) (@exec_impure i a).
-
-Next Obligation.
-  add_morphism_tactic.
-  intros sem sem' equ1 p q equ2.
-  unfold exec_impure.
-  now rewrite equ1, equ2.
-Qed.
-
-Lemma run_impure_equiv {i a} (p q : impure i a) (equ : p == q) (sem : semantics i)
-  : run_impure sem p == run_impure sem q.
-Proof.
-  now rewrite equ.
-Qed.
-
-Hint Resolve run_impure_equiv : freespec.
-
-Lemma run_impure_exec_impure_equiv {i a}
-  (sem sem' : semantics i) (p q : impure i a) (equ : run_impure sem p == run_impure sem' q)
-  : exec_impure sem p == exec_impure sem' q.
-Proof.
-  now inversion equ; ssubst.
-Qed.
-
-Hint Resolve run_impure_exec_impure_equiv : freespec.
-
-Lemma run_impure_eval_impure_equiv {i a}
-  (sem sem' : semantics i) (p q : impure i a) (equ : run_impure sem p == run_impure sem' q)
-  : eval_impure sem p = eval_impure sem' q.
-Proof.
-  now inversion equ; ssubst.
-Qed.
-
-Hint Resolve run_impure_eval_impure_equiv : freespec.
-
-Lemma exec_impure_equiv {i a} (p q : impure i a) (equ : p == q) (sem : semantics i)
-  : exec_impure sem p == exec_impure sem q.
-Proof.
-  now rewrite equ.
-Qed.
-
-Hint Resolve run_impure_equiv : freespec.
-
-Lemma impure_bind_equation {i a b}
-  (p : impure i a) (f : a -> impure i b) (sem : semantics i)
-  : run_impure sem (impure_bind p f)
-    == run_impure (exec_impure sem p) (f (eval_impure sem p)).
-Proof.
-  revert sem.
-  induction p; intros sem.
-  + reflexivity.
-  + cbn.
-    apply H.
-Qed.
-
-(** * Component
-
-    In FreeSpec, we call a component an entity which exposes an interface [i],
-    and uses primitives of an interface [j] to compute the result of primitives
-    of [i].  Besides, a component is likely to carry its own internal state (of
-    type [s]).
-
-<<
-                               c : component i j s
-                           i +---------------------+      j
-                           | |                     |      |
-                   +------>| |       st : s        |----->|
-                           | |                     |      |
-                             +---------------------+
->>
-
-    Thus, a component [c : component i j s] is a polymorphic function which,
-    given a primitive of [i], and the current state of the component, maps
-    impure computations which return the result of the primitive and the new
-    state of the component.  We use the State monad [state_t] to handle the
-    internal state of the component more easily.  We could have use the [STORE
-    s] interface discussed previously, but we believe using [state_t] simplifies
-    the reasoning process of FreeSpec. *)
-
-Definition component (i j : interface) : Type :=
-  forall (a : Type), i a -> impure j a.
-
-(** The similarity between FreeSpec components and operational semantics may be
-    confusing at first.  The main difference between the two concepts is simple:
-    operational semantics are self-contained terms which can, alone, be used to
-    interpret impure computations of a given interface.  Components, on the
-    other hand, are not self-contained.  Without an intial state [init : s] and
-    an operational semantics for [j], we cannot use a component [c : component i
-    j s] to interpret an impure computation using [i].
-
-    Given an initial state and and initial semantics for [j], we can however
-    derive an operational semantics for [i] from a component [c]. *)
-
-CoFixpoint derive_semantics {i j} (c : component i j) (sem : semantics j)
-  : semantics i :=
-  mk_semantics (fun (a : Type) (p : i a) =>
-                  let run := run_impure sem (c a p) in
-                  let res := interp_result run in
-                  let next := interp_next run in
-                  mk_out res (derive_semantics c next)).
-
-(** So, [⊕] on the one hand allows for composing operational semantics
-    horizontally, and [derive_semantics] allows for composing components
-    vertically.  Using these two operators, we can model a complete system in a
-    modular manner, by defining each of its component independently, then
-    composing them together with [⊕] and [derive_semantics]. *)
-
-Definition bootstrap {i} (c : component i <>) : semantics i :=
-  derive_semantics c semempty.
