stdlib/theories/Stdlib/Raise.v
@@ -1,36 +1,39 @@
 From FreeSpec Require Import Core.
 
-Generalizable All Variables.
-
-Class Into (a b : Type) :=
-  { into : a -> b
+Class Into (α β : Type) :=
+  { into : α -> β
   }.
 
-Instance refl_Into (a : Type) : Into a a :=
+Instance refl_Into (α : Type) : Into α α :=
   { into := fun x => x
   }.
 
-Inductive RAISE (a : Type) : interface :=
-| Raise {b} (x : a) : RAISE a b.
+Inductive RAISE (α : Type) : interface :=
+| Raise {β} (x : α) : RAISE α β.
 
-Arguments Raise [a b] x.
+Arguments Raise [α β] x.
 
-Definition raise `{Into c a, Provide ix (RAISE a)} {b} (x : c) : impure ix b :=
+Definition raise `{Into δ α, Provide ix (RAISE α)} {β} (x : δ) : impure ix β :=
   request (Raise (into x)).
 
-Definition try `{Into c a, Provide ix (RAISE a)} {b} (p : impure ix (c + b)) : impure ix b :=
-  do var res <- p in
+Definition try `{Into δ α, Provide ix (RAISE α)} {β} (p : impure ix (δ + β)) : impure ix β :=
+  do let* res <- p in
      match res with
      | inl e => raise e
      | inr x => pure x
      end
   end.
 
-Fixpoint recover {ix a b} (p : impure (ix ⊕ RAISE a) b) (h : a -> impure ix b) : impure ix b :=
+Fixpoint recover {ix α β} (p : impure (ix + RAISE α) β) (h : α -> impure ix β) : impure ix β :=
   match p with
   | local x => local x
   | request_then (in_right (Raise e)) _ => h e
   | request_then (in_left e) f => request_then e (fun x => recover (f x) h)
   end.
 
-Notation "'recover' p 'with'  v 'of' t '=>' h 'end'" := (recover p (fun (v : t) => h)).
+Declare Scope raise_scope.
+
+Notation "'recover' p 'with'  v 'of' t '=>' h 'end'" :=
+  (recover p (fun (v : t) => h)) : raise_scope.
+
+Open Scope raise_scope.
