core/tests/provide_notation.v
@@ -18,8 +18,7 @@
  * along with this program. If not, see <http://www.gnu.org/licenses/>.
  *)
 
-From FreeSpec Require Import Core Notations.
-Generalizable All Variables.
+From FreeSpec Require Import Core.
 
 Axioms (i1 i2 i3 i4 : interface).
 
@@ -30,7 +29,7 @@ Definition p `{Provide4 ix i1 i4 i3 i2} : impure ix nat :=
   do p1; p2 end.
 
 Definition provide_notation_test_1 {a} `{StrictProvide3 ix i1 i2 i3} (p : i2 a) : ix a :=
-  lift_eff p.
+  inj_p p.
 
 Lemma provide_notation_test_2 `{StrictProvide3 ix i1 i2 i3} : StrictProvide2 ix i2 i3.
 
@@ -38,16 +37,16 @@ Proof.
   typeclasses eauto.
 Qed.
 
-Definition provide_notation_test_3 {a} (i1 i2 i3 : interface) (p : i2 a) : (i1 ⊕ i2 ⊕ i3) a :=
-  lift_eff p.
+Definition provide_notation_test_3 {a} (i1 i2 i3 : interface) (p : i2 a) : (iplus (iplus i1 i2) i3) a :=
+  inj_p p.
 
-Lemma provide_notation_test_4 (i1 i2 i3 : interface) : Provide (i1 ⊕ (i2 ⊕ i3)) i2.
+Lemma provide_notation_test_4 (i1 i2 i3 : interface) : Provide (i1 + (i2 + i3)) i2.
 
 Proof.
   typeclasses eauto.
 Qed.
 
-Lemma provide_notation_test_5 (i1 i2 i3 : interface) : StrictProvide2 (i1 ⊕ i2 ⊕ i3) i2 i1.
+Lemma provide_notation_test_5 (i1 i2 i3 : interface) : StrictProvide2 (i1 + i2 + i3) i2 i1.
 
 Proof.
   typeclasses eauto.
