core/theories/Core/Component.v
@@ -1,0 +1,72 @@
+(* FreeSpec
+ * Copyright (C) 2018–2019 ANSSI
+ *
+ * Contributors:
+ * 2018–2019 Thomas Letan <thomas.letan@ssi.gouv.fr>
+ *
+ * This impure is free software: you can redistribute it and/or modify
+ * it under the terms of the GNU General Public License as published by
+ * the Free Software Foundation, either version 3 of the License, or
+ * (at your option) any later version.
+ *
+ * This impure is distributed in the hope that it will be useful,
+ * but WITHOUT ANY WARRANTY; without even the implied warranty of
+ * MERCHANTABILITY or FITNESS FOR A PARTICULAR PURPOSE.  See the
+ * GNU General Public License for more details.
+ *
+ * You should have received a copy of the GNU General Public License
+ * along with this program. If not, see <http://www.gnu.org/licenses/>.
+ *)
+
+From FreeSpec.Core Require Import Interface Semantics Impure.
+
+(** * Component
+
+    In FreeSpec, a _component_ an entity which exposes an interface [i],
+    and uses primitives of an interface [j] to compute the result of primitives
+    of [i].  Besides, a component is likely to carry its own internal state (of
+    type [s]).
+
+<<
+                               c : component i j s
+                           i +---------------------+      j
+                           | |                     |      |
+                   +------>| |       st : s        |----->|
+                           | |                     |      |
+                             +---------------------+
+>>
+
+    Thus, a component [c : component i j] is a polymorphic function which
+    maps primitive of [i] to impure computations using [j]. *)
+
+Definition component (i j : interface) : Type :=
+  forall (α : Type), i α -> impure j α.
+
+(** The similarity between FreeSpec components and operational semantics may be
+    confusing at first. The main difference between the two concepts is simple:
+    operational semantics are self-contained terms which can, alone, be used to
+    interpret impure computations of a given interface.  Components, on the
+    other hand, are not self-contained.  Without an operational semantics for
+    [j], we cannot use a component [c : component i j] to interpret an impure
+    computation using [i].
+
+    Given an initial semantics for [j], we can however derive an operational
+    semantics for [i] from a component [c]. *)
+
+CoFixpoint derive_semantics {i j} (c : component i j) (sem : semantics j)
+  : semantics i :=
+  mk_semantics (fun _ p =>
+                  let run := run_impure sem (c _ p) in
+                  let res := interp_result run in
+                  let next := interp_next run in
+                  mk_out res (derive_semantics c next)).
+
+(** So, [⊕] on the one hand allows for composing operational semantics
+    horizontally, and [derive_semantics] allows for composing components
+    vertically.  Using these two operators, we can model a complete system in a
+    hierarchical and modular manner, by defining each of its component
+    independently, then composing them together with [⊕] and
+    [derive_semantics]. *)
+
+Definition bootstrap {i} (c : component i iempty) : semantics i :=
+  derive_semantics c iempty_semantics.
