core/theories/Core/Contract.v
@@ -1,0 +1,713 @@
+(* FreeSpec
+ * Copyright (C) 2018–2019 ANSSI
+ *
+ * Contributors:
+ * 2018–2019 Thomas Letan <thomas.letan@ssi.gouv.fr>
+ *
+ * This program is free software: you can redistribute it and/or modify
+ * it under the terms of the GNU General Public License as published by
+ * the Free Software Foundation, either version 3 of the License, or
+ * (at your option) any later version.
+ *
+ * This program is distributed in the hope that it will be useful,
+ * but WITHOUT ANY WARRANTY; without even the implied warranty of
+ * MERCHANTABILITY or FITNESS FOR A PARTICULAR PURPOSE.  See the
+ * GNU General Public License for more details.
+ *
+ * You should have received a copy of the GNU General Public License
+ * along with this program. If not, see <http://www.gnu.org/licenses/>.
+ *)
+
+(** In this library, we provide the necessary material to reason about FreeSpec
+    component both in isolation, and in composition.  To do that, we focus our
+    reasoning principle on interfaces, by defining how their primitives shall be
+    used in the one hand, and what to expect the result computed by “correct”
+    operational semantics (according to a certain definition of “correct”). *)
+
+
+From Prelude Require Import All.
+From Coq Require Import Setoid Morphisms.
+From FreeSpec.Core Require Export Interface Impure Semantics Component.
+
+#[local]
+Open Scope signature_scope.
+
+(** * Definition *)
+
+(** A contract dedicated to [i : interface] primilarly provides two
+    predicates.
+
+    - [caller_obligation] distinguishes between primitives that can be used (by
+      an impure computation), and primitives that cannot be used.
+    - [callee_obligation] specifies which guarantee can be expected from
+      primitives results, as computed by a “good” operational semantics.
+
+    Both [caller_obligation] and [callee_obligation] models properties that may
+    vary in time, e.g., a primitive may be forbidden at a given time, but
+    authorized later.  To take this possibility into account, contracts are
+    parameterized by what we have called a “witness.”  A witness is a term which
+    describes the necessary information of the past, and allows for taking
+    decision for the present.  It can be seen as an abstraction of the concrete
+    state of the interface implementor.
+
+    To keep this state up-to-date after each primitive interpretation,
+    contracts also define a dedicated function [witness_update]. *)
+
+Record contract (i : interface) (Ω : Type) : Type := make_contract
+  { witness_update (ω : Ω) : forall (α : Type), i α -> α -> Ω
+  ; caller_obligation (ω : Ω) : forall (α : Type),  i α -> Prop
+  ; callee_obligation (ω : Ω) : forall (α : Type), i α -> α -> Prop
+  }.
+
+Declare Scope contract_scope.
+Bind Scope contract_scope with contract.
+
+Arguments make_contract [i Ω] (_ _ _).
+Arguments witness_update [i Ω] (c ω) [α] (_ _).
+Arguments caller_obligation [i Ω] (c ω) [α] (_).
+Arguments callee_obligation [i Ω] (c ω) [α] (_ _).
+
+(** The most simple contract we can define is the one that requires
+    anything both for the impure computations which uses the primitives of a
+    given interface, and for the operational semantics which compute results for
+    these primitives. *)
+
+Definition const_witness {i} :=
+  fun (u : unit) (α : Type) (e : i α) (x : α) => u.
+
+Definition no_caller_obligation {i Ω} (ω : Ω) (α : Type) (e : i α) : Prop := True.
+
+Definition no_callee_obligation {i Ω} (ω : Ω) (α : Type) (e : i α) (x : α) : Prop := True.
+
+Definition no_contract (i : interface) : contract i unit :=
+  {| witness_update := const_witness
+   ; caller_obligation := no_caller_obligation
+   ; callee_obligation := no_callee_obligation
+   |}.
+
+(** A similar —and as simple— contract is the one that forbids the use of a
+    given interface. *)
+
+Definition do_no_use {i Ω} (ω : Ω) (α : Type) (e : i α) : Prop := False.
+
+Definition forbid_specs (i : interface) : contract i unit :=
+  {| witness_update := const_witness
+   ; caller_obligation := do_no_use
+   ; callee_obligation := no_callee_obligation
+   |}.
+
+(** As we compose interfaces and operational semantics, we can easily compose
+    contracts together, by means of the [cplus] operator. Given [i] and [j]
+    two interfaces, if we can reason about [i] and [j] independently (e.g., the
+    caller obligations of [j] do not vary when we use [i]), then we can compose
+    [ci : contract i Ωi] and [cj : contract j Ωj], such that [cplus ci cj] in a
+    contract for [i + j]. *)
+
+Definition gen_witness_update `{MayProvide ix i} {Ω α} (c : contract i Ω)
+    (ω :  Ω) (e : ix α) (x : α)
+  : Ω :=
+  match proj_p e with
+  | Some e => witness_update c ω e x
+  | None => ω
+  end.
+
+Definition gen_caller_obligation `{MayProvide ix i} {Ω α} (c : contract i Ω)
+    (ω :  Ω) (e : ix α)
+  : Prop :=
+  match proj_p e with
+  | Some e => caller_obligation c ω e
+  | None => True
+  end.
+
+Definition gen_callee_obligation `{MayProvide ix i} {Ω α} (c : contract i Ω)
+    (ω :  Ω) (e : ix α) (x : α)
+  : Prop :=
+  match proj_p e with
+  | Some e => callee_obligation c ω e x
+  | None => True
+  end.
+
+Definition cplus `{Provide ix i, Provide ix j} {Ωi Ωj}
+    (ci : contract i Ωi) (cj : contract j Ωj)
+  : contract ix (Ωi * Ωj) :=
+  {| witness_update := fun (ω : Ωi * Ωj) (α : Type) (e : ix α) (x : α) =>
+                         (gen_witness_update ci (fst ω) e x, gen_witness_update cj (snd ω) e x)
+  ;  caller_obligation := fun (ω : Ωi * Ωj) (α : Type) (e : ix α) =>
+                       gen_caller_obligation ci (fst ω) e /\ gen_caller_obligation cj (snd ω) e
+  ;  callee_obligation := fun (ω : Ωi * Ωj) (α : Type) (e : ix α) (x : α) =>
+                   gen_callee_obligation ci (fst ω) e x /\ gen_callee_obligation cj (snd ω) e x
+  |}.
+
+Infix "+" := cplus : contract_scope.
+
+(** Finally, and as an example, we define a contract for the interface
+    [STORE s] we discuss in [FreeSpec.Core.Impure].  As a reminder, the
+    interface is defined as follows:
+
+<<
+Inductive STORE (s : Type) : interface :=
+| Get : STORE s s
+| Put (x : s) : STORE s unit.
+>>
+
+    For [STORE s], the best witness is the actual value of the mutable
+    variable.  Therefore, the contract for [STORE s] may be [specs (STORE
+    s) s], and the witness will be updated after each [Put] call. *)
+
+Definition store_update (s : Type) :=
+  fun (x : s) (α : Type) (e : STORE s α) (_ : α) =>
+    match e with
+    | Get => x
+    | Put x' => x'
+    end.
+
+(** Assuming the mutable variable is being initialized prior to any impure
+    computation interpretation, we do not have any obligations over the use of
+    [STORE s] primitives.  We will get back to this assertion once we have
+    defined our contract, but in the meantime, we define its callee obligation.
+
+    The logic of these callee obligations is as follows: [Get] is expected to
+    produce a result strictly equal to the witness, and we do not have any
+    obligations about the result of [Put] (which belongs to [unit] anyway, so
+    there is not much to tell). *)
+
+Inductive o_callee_store (s : Type) (x : s) : forall (α : Type), STORE s α -> α -> Prop :=
+| get_o_callee (x' : s) (equ : x = x') : o_callee_store s x s Get x'
+| put_o_callee (x' : s) (u : unit) : o_callee_store s x unit (Put x') u.
+
+(** The actual contract can therefore be defined as follows: *)
+
+Definition store_specs (s : Type) : contract (STORE s) s :=
+  {| witness_update := store_update s
+  ;  caller_obligation := no_caller_obligation
+  ;  callee_obligation := o_callee_store s
+  |}.
+
+(** Now, as we briefly mentionned, this contract allows for reasoning about
+    an impure computation which uses the [STORE s] interface, assuming the
+    mutable, global variable has been initialized.  We can define another
+    contract that does not rely on such assumption, and on the contrary,
+    requires an impure computation to initialize the variable prior to using it.
+
+    In this context, the witness can solely be a boolean which tells if the
+    variable has been initialized, and the [callee_obligation] will require the
+    witness to be [true] to authorize a call of [Get].
+
+    This is one of the key benefit of the FreeSpec approach: because the
+    contracts are defined independently from impure computation and
+    interfaces, we can actually define several contracts to consider
+    different set of hypotheses. *)
+
+(** * Reasoning with Contracts *)
+
+(** ** Impure Computation Trustworthiness *)
+
+(** An impure computation [p] is said respectful wrt. a contract [c] in
+    accordance to a witness [ω] when it only uses primitives of [i] which
+    satisfies [c] obligations. *)
+
+Inductive respectful_impure `{MayProvide ix i} {α Ω} (c : contract i Ω) (ω : Ω) : impure ix α -> Prop :=
+
+(** - Given a term [x], the computation [local x] is always respectful wrt. [c]
+      in accordance to [ω], since it does not use any primitives. *)
+
+| respectful_local (x : α)
+  : respectful_impure c ω (local x)
+
+(** - Given a primitive [e] and a continuation [f], if
+
+      - [e] satisfies [c] caller obligation
+      - [f] computations are respectful wrt. [c] in accordance to [ω'], where
+        [ω'] is the witness updated after [e] interpretation
+
+      then the impure computation [request_then e f] is respectful wrt. [c] in
+      accordance to [ω]. *)
+
+| respectful_request_some {β}
+    (e : ix β) (f : β -> impure ix α)
+    (req : gen_caller_obligation c ω e)
+    (next : forall (x : β),
+        gen_callee_obligation c ω e x
+        -> respectful_impure c (gen_witness_update c ω e x) (f x))
+  : respectful_impure c ω (request_then e f).
+
+#[program]
+Instance respectful_impure_Proper : Proper ('equal ==> Basics.impl) (@respectful_impure ix i H α Ω c ω).
+
+Next Obligation.
+  add_morphism_tactic.
+  unfold Basics.impl.
+  intros p q equ.
+  revert ω.
+  induction equ; intros ω.
+  + auto.
+  + intros trust.
+    inversion trust; ssubst.
+    constructor.
+    ++ exact req.
+    ++ intros x q.
+       apply H0.
+       now apply next.
+Qed.
+
+(** As is, the definition of [respectful_impure] would force FreeSpec users to
+    unfold any impure computations they may combine together with [bind].  For
+    instance, proving a computation of the form [bind p (λ _, p)] is respectful
+    would require to prove [p] is respectful twice, for two different
+    witnesses.  Moreover, it could be challenging to know, when interactively
+    writing the proof script, when “the first [p]” stops, and when “the second
+    [p]” starts.
+
+    We need a way to compose proofs about impure computations the same way we
+    compose impure computations with [bind].  We do that with the
+    [respectful_run] predicate, which describes the potential outcomes of a
+    computation in terms of results and witnesses. *)
+
+Inductive respectful_run `{MayProvide ix i} {α Ω} (c : contract i Ω)
+  : impure ix α -> Ω -> Ω -> α -> Prop :=
+
+(** Given a term [x], and an initial witness [ω], then a respectful run of
+    [local x] produced a result [x] and a witness state [ω]. *)
+
+| run_local (x : α) (ω : Ω)
+  : respectful_run c (local x) ω ω x
+
+(** Given an initial witness [ω], a primitive [e] which satisfies [c]
+    caller obligations, and a continuation [f], a result [x] for [e] which
+    satisfies [c] callee obligations, if we can show that there is a respectful
+    run of [f x] which produces a term [y] and a witness [ω'], then there is a
+    respectful run of [request_then e f] which produces a result [y] and a
+    witness [ω']. *)
+
+| run_request {β} (ω : Ω)
+    (e : ix β) (o_caller : gen_caller_obligation c ω e) (f : β -> impure ix α)
+    (x : β) (o_callee : gen_callee_obligation c ω e x)
+    (ω' : Ω) (y : α) (rec : respectful_run c (f x) (gen_witness_update c ω e x) ω' y)
+  : respectful_run c (request_then e f) ω ω' y.
+
+(** Given a contract [c] and a witness [ω] an impure computation [p] and a
+    continuation [f] if
+
+    - [p] is a respectful impure computation wrt. [c] in accordance to [ω], and
+    - for all result [x] and witness [ω'] produces by [p], [f x] is respectful,
+
+    then [bind p f] is respectful. *)
+
+Lemma respectful_bind_respectful_run `{MayProvide ix i} {α β Ω}
+  (c : contract i Ω) (ω : Ω)
+  (p : impure ix α) (f : α -> impure ix β)
+  (respect : respectful_impure c ω p)
+  (run : forall (x : α) (ω' : Ω),
+      respectful_run c p ω ω' x -> respectful_impure c ω' (f x))
+  : respectful_impure c ω (impure_bind p f).
+
+Proof.
+  revert ω respect run.
+  induction p; intros ω respect run.
+  + apply run.
+    constructor.
+  + cbn.
+    inversion respect; ssubst.
+    constructor.
+    ++ apply req.
+    ++ intros y o_callee_x.
+       apply H0; [ auto |].
+       intros z ω' run'.
+       apply run.
+       econstructor; eauto.
+Qed.
+
+Hint Resolve respectful_bind_respectful_run : freespec.
+
+Lemma respectful_bind_exists_respectful_run `{MayProvide ix i} {α β Ω}
+    (c : contract i Ω) (ω ω' : Ω)
+    (p : impure ix α) (f : α -> impure ix β) (x : β)
+    (respect : respectful_run c (impure_bind p f) ω ω' x)
+  : exists (ω'' : Ω) (y : α),
+    respectful_run c p ω ω'' y /\ respectful_run c (f y) ω'' ω' x.
+
+Proof.
+  revert respect.
+  revert ω ω'.
+  induction p; intros ω ω' respect.
+  + exists ω; exists x0.
+    split.
+    ++ constructor.
+    ++ exact respect.
+  + inversion respect; ssubst.
+    apply H0 in rec.
+    destruct rec as [ω'' [y [trust1 trust2]]].
+    exists ω''; exists y.
+    split; auto.
+    constructor 2 with (x := x0); auto.
+Qed.
+
+#[program]
+Instance respectful_run_Proper
+  : Proper ('equal ==> eq ==> eq ==> eq ==> Basics.impl) (@respectful_run ix i H α Ω c).
+
+Next Obligation.
+  add_morphism_tactic.
+  unfold Basics.impl.
+  intros p q equ.
+  induction equ.
+  + intros ω ω' y run.
+    now inversion run; subst.
+  + intros ω ω' y run.
+    inversion run; ssubst.
+    constructor 2 with (x := x).
+    ++ auto.
+    ++ auto.
+    ++ now apply H0.
+Qed.
+
+(** ** Semantics Compliance *)
+
+(** Given a semantics [sem], and a witness [ω] if [sem] computes results which
+    satisfies [c] callee obligations for effects which satisfy [c] caller
+    obligations and if the resulting semantics produces after interpreting [e]
+    complies to [c] in accordance to [ω'], where [ω'] is the new witness state
+    after [e] interpretation then [sem] complies to [c] in accordance to [ω] *)
+
+CoInductive compliant_semantics `{MayProvide ix i} {Ω} (c : contract i Ω) : Ω -> semantics ix -> Prop :=
+| compliant_semantics_rec
+    (sem : semantics ix) (ω : Ω)
+    (o_callee : forall {α} (e : ix α),
+        gen_caller_obligation c ω e -> gen_callee_obligation c ω e (eval_effect sem e))
+    (next : forall {α} (e : ix α),
+        gen_caller_obligation c ω e
+        -> compliant_semantics c (gen_witness_update c ω e (eval_effect sem e)) (exec_effect sem e))
+  : compliant_semantics c ω sem.
+
+(** Proving that semantics obtained from the [store] function are compliant with
+    [store_specs] is relatively simple. *)
+
+Lemma store_complies_to_store_specs {s} (st : s)
+  : compliant_semantics (store_specs s) st (store st).
+
+Proof.
+  revert st; cofix compliant_semantics_rec; intros st.
+  constructor.
+  + intros a [|st'] _.
+    ++ now constructor.
+    ++ now constructor.
+  + intros a e req.
+    cbn.
+    assert (R : exec_effect (store st) e = store (store_update s st a e (eval_effect (store st) e)))
+      by now destruct e as [|st'].
+    rewrite R.
+    apply compliant_semantics_rec.
+Qed.
+
+Lemma compliant_semantics_caller_obligation_callee_obligation `{MayProvide ix i} {Ω α} (c : contract i Ω) (ω : Ω)
+  (e : ix α) (o_caller : gen_caller_obligation c ω e)
+  (sem : semantics ix) (comp : compliant_semantics c ω sem)
+  : gen_callee_obligation c ω e (eval_effect sem e).
+
+Proof.
+  inversion comp; ssubst.
+  now apply o_callee.
+Qed.
+
+Hint Resolve compliant_semantics_caller_obligation_callee_obligation : freespec.
+
+Lemma compliant_semantics_caller_obligation_compliant `{MayProvide ix i} {Ω α} (c : contract i Ω) (ω : Ω)
+  (e : ix α) (o_caller : gen_caller_obligation c ω e)
+  (sem : semantics ix) (comp : compliant_semantics c ω sem)
+  : compliant_semantics c (gen_witness_update c ω e (eval_effect sem e)) (exec_effect sem e).
+
+Proof.
+  inversion comp; ssubst.
+  now apply next.
+Qed.
+
+Hint Resolve compliant_semantics_caller_obligation_compliant : freespec.
+
+Lemma compliant_semantics_exec_effect_equ `{MayProvide ix i} {Ω α} (c : contract i Ω) (ω : Ω)
+  (sem sem' : semantics ix) (equ : sem == sem')
+  (e : ix α)
+  : exec_effect sem e == exec_effect sem' e.
+
+Proof.
+  inversion equ; ssubst.
+  specialize step_equiv with α e.
+  now inversion step_equiv; ssubst.
+Qed.
+
+Hint Resolve compliant_semantics_exec_effect_equ : freespec.
+
+#[program]
+Instance compliant_semantics_Proper : Proper ('equal ==> Basics.impl) (@compliant_semantics ix i H Ω c ω).
+
+Next Obligation.
+  add_morphism_tactic.
+  revert ω.
+  cofix compliant_semantics_Proper; intros ω.
+  intros σ σ' equ comp.
+  destruct comp.
+  constructor.
+  + now setoid_rewrite <- equ.
+  + intros a e o_caller.
+    apply (compliant_semantics_Proper (gen_witness_update c ω e (eval_effect σ' e)) (exec_effect sem e)).
+    ++ auto with freespec.
+    ++ rewrite <- equ at 1.
+       now apply next.
+Qed.
+
+Lemma no_contract_compliant_semantics `{MayProvide ix i} (sem : semantics ix) (u : unit)
+  : compliant_semantics (no_contract i) u sem.
+
+Proof.
+  revert sem.
+  cofix no_contract_compliant_semantics; intros sem.
+  constructor.
+  + trivial.
+  + intros α e req.
+    unfold gen_witness_update.
+    destruct (proj_p e); [ apply no_contract_compliant_semantics | auto ].
+Qed.
+
+Hint Resolve no_contract_compliant_semantics : freespec.
+
+#[local]
+Fixpoint witness_impure_aux `{MayProvide ix i} {Ω α}
+  (sem : semantics ix) (p : impure ix α) (c : contract i Ω) (ω : Ω) : interp_out ix α * Ω :=
+  match p with
+  | local x => (mk_out x sem, ω)
+  | request_then e f =>
+    let out := run_effect sem e in
+    let res := interp_result out in
+    witness_impure_aux (interp_next out) (f res) c (gen_witness_update c ω e res)
+  end.
+
+#[program]
+Instance witness_impure_aux_Proper_2
+  : Proper (eq ==> 'equal ==> eq ==> eq ==> eq) (@witness_impure_aux ix i H Ω a).
+
+Next Obligation.
+  add_morphism_tactic.
+  intros sem p q equp c ω.
+  revert sem ω.
+  induction equp; intros sem ω.
+  + reflexivity.
+  + cbn.
+    apply H0.
+Qed.
+
+Lemma fst_witness_impure_aux_run_impure `{MayProvide ix i} {Ω α}
+  (sem : semantics ix) (p : impure ix α) (c : contract i Ω) (ω : Ω)
+  : fst (witness_impure_aux sem p c ω) = run_impure sem p.
+
+Proof.
+  revert sem ω.
+  induction p; intros sem ω.
+  + reflexivity.
+  + apply H0.
+Qed.
+
+Hint Rewrite @fst_witness_impure_aux_run_impure : freespec.
+
+Definition witness_impure `{MayProvide ix i} {Ω α}
+  (sem : semantics ix) (p : impure ix α) (c : contract i Ω) (ω : Ω) : Ω :=
+  snd (witness_impure_aux sem p c ω).
+
+#[program]
+Instance witness_impure_Proper
+  : Proper (eq ==> 'equal ==> eq ==> eq ==> eq) (@witness_impure ix i H Ω α).
+
+Next Obligation.
+  add_morphism_tactic.
+  unfold witness_impure.
+  intros sem p q equp c ω.
+  now rewrite equp.
+Qed.
+
+Lemma compliant_semantics_respectful_impure_gives_respectful_run `{MayProvide ix i} {Ω α}
+  (c : contract i Ω) (ω : Ω) (p : impure ix α) (trust : respectful_impure c ω p)
+  (sem : semantics ix) (comp : compliant_semantics c ω sem)
+  : respectful_run c p ω (witness_impure sem p c ω) (eval_impure sem p).
+
+Proof.
+  revert sem comp trust. revert ω.
+  induction p; intros ω sem comp trust.
+  + constructor.
+  + inversion trust; ssubst.
+    inversion comp; ssubst.
+    econstructor; auto.
+    apply H0.
+    ++ now apply next0.
+    ++ inversion trust; ssubst.
+       apply next1.
+       now apply o_callee.
+Qed.
+
+Hint Resolve compliant_semantics_respectful_impure_gives_respectful_run : freespec.
+
+Lemma witness_impure_request_then_equ `{MayProvide ix i} {Ω α β} (c : contract i Ω) (ω : Ω)
+  (sem : semantics ix) (e : ix α) (f : α -> impure ix β)
+  : witness_impure sem (request_then e f) c ω
+    = witness_impure (exec_effect sem e)
+                     (f (eval_effect sem e))
+                     c
+                     (gen_witness_update c ω e (eval_effect sem e)).
+
+Proof eq_refl.
+
+Hint Rewrite @witness_impure_request_then_equ : freespec.
+
+Lemma respectful_impure_compliant_specs `{MayProvide ix i} {Ω α} (c : contract i Ω) (ω : Ω)
+  (p : impure ix α) (trust : respectful_impure c ω p)
+  (sem : semantics ix) (comp : compliant_semantics c ω sem)
+  : compliant_semantics c (witness_impure sem p c ω) (exec_impure sem p).
+
+Proof.
+  revert trust sem comp. revert ω.
+  induction p; intros ω trust sem comp.
+  + exact comp.
+  + inversion trust; ssubst.
+    autorewrite with freespec.
+    apply H0; auto with freespec.
+Qed.
+
+Hint Resolve respectful_impure_compliant_specs : freespec.
+
+Lemma gen_callee_obligation_equ {α Ωi Ωj} `{Provide ix i} `{Provide ix j}
+    (ci : contract i Ωi) (ωi : Ωi)
+    (cj : contract j Ωj) (ωj : Ωj)
+    (e : ix α) (x : α)
+  : gen_callee_obligation ci ωi e x /\ gen_callee_obligation cj ωj e x
+    <-> gen_callee_obligation (ci + cj) (ωi, ωj) e x.
+
+Proof.
+  split; auto.
+Qed.
+
+Lemma gen_caller_obligation_equ {α Ωi Ωj} `{Provide ix i} `{Provide ix j}
+    (ci : contract i Ωi) (ωi : Ωi) (cj : contract j Ωj) (ωj : Ωj) (e : ix α)
+  : gen_caller_obligation ci ωi e /\ gen_caller_obligation cj ωj e
+    <-> gen_caller_obligation (ci + cj) (ωi, ωj) e.
+
+Proof.
+  split; auto.
+Qed.
+
+Lemma respectful_impure_generalize `{Provide ix i} `{Provide ix j} {α Ωi Ωj}
+    (p : impure ix α)
+    (ci : contract i Ωi) (ωi : Ωi) (cj : contract j Ωj) (ωj : Ωj)
+  : respectful_impure ci ωi p
+    -> respectful_impure cj ωj p
+    -> respectful_impure (ci + cj) (ωi, ωj) p.
+
+Proof.
+  revert ωi ωj.
+  induction p; intros ωi ωj.
+  + intros.
+    constructor.
+  + intros trust trust'.
+    inversion trust; ssubst.
+    inversion trust'; ssubst.
+    constructor.
+    ++ rewrite <- gen_caller_obligation_equ.
+       now split.
+    ++ intros x o_callee.
+       rewrite <- gen_callee_obligation_equ in o_callee.
+       apply H3; [ apply next | apply next0 ]; apply o_callee.
+Qed.
+
+(** ** Component Correctness *)
+
+(** We consider a component [c : component i j s], meaning [c] exposes an
+    interface [i], uses an interface [j], and carries an internal state of type
+    [s].
+
+<<
+                            c : component i j s
+                        i +---------------------+      j
+                        | |                     |      |
+                +------>| |       st : s        |----->|
+                        | |                     |      |
+                          +---------------------+
+>>
+
+    We say [c] is correct wrt. [ci] (a contract for [i]) and [cj] (a contract
+    for [i]) iff given primitives which satisfies the caller obligation of [ci],
+    [c] will
+
+    - use respectful impure computations wrt. [cj]
+    - compute results which satisfy [ci] callee obligations, assuming it can
+      rely on a semantics of [j] which complies with [cj]
+
+    The two witness states [ωi : Ωi] (for [speci]) and [ωj : Ωj] (for [specj]),
+    and [st : s] the internal state of [c] remained implicit in the previous
+    sentence.  In practice, we associate them together by means of a dedicated
+    predicate [pred].  It is expected that [pred] is an invariant throughout
+    [c]'s life, meaning that as long as [c] computes result for legitimate
+    effects (wrt.  [speci] effects, the updated values of [ωi], [ωj] and [st]
+    continue to satisfy [pred]. *)
+
+Definition correct_component {i jx Ωi Ωj}
+  (c : component i jx) `{MayProvide jx j}
+  (ci : contract i Ωi) (cj : contract j Ωj)
+  (pred : Ωi -> Ωj -> Prop) : Prop :=
+  forall (ωi : Ωi) (ωj : Ωj) (init : pred ωi ωj)
+    (α : Type) (e : i α) (o_caller : caller_obligation ci ωi e),
+    respectful_impure cj ωj (c α e) /\
+    forall (x : α) (ωj' : Ωj)
+      (run : respectful_run cj (c α e) ωj ωj' x),
+      callee_obligation ci ωi e x /\ pred (witness_update ci ωi e x) ωj'.
+
+(** Once we have proven [c] is correct wrt. to [speci] and [specj] with [pred]
+    acting as an invariant throughout [c] life, we show we can derive a
+    semantics from [c] with an initial state [st] which complies to [speci] in
+    accordance to [ωi] if we use a semantics of [j] which complies to [specj] in
+    accordance to [ωj], where [pred ωi st ωj] is satisfied. *)
+
+Lemma respectful_impure_compliant_specs_respectful_run `{MayProvide ix i} {a Ω}
+    (spec : contract i Ω) (ω : Ω)
+    (sem : semantics ix) (comp : compliant_semantics spec ω sem)
+    (p : impure ix a) (trust : respectful_impure spec ω p)
+  : respectful_run spec p ω (witness_impure sem p spec ω) (eval_impure sem p).
+
+Proof.
+  revert ω sem comp trust.
+  induction p; intros ω sem comp trust.
+  + constructor.
+  +  inversion trust; ssubst.
+     constructor 2 with (x := eval_effect sem e).
+     ++ exact req.
+     ++ auto with freespec.
+     ++ change (witness_impure sem (request_then e f) spec ω)
+          with (witness_impure (exec_effect sem e) (f (eval_effect sem e)) spec
+                               (gen_witness_update spec ω e (eval_effect sem e))).
+        change (eval_impure sem (request_then e f))
+          with (eval_impure (exec_effect sem e) (f (eval_effect sem e))).
+        apply H0;
+          auto with freespec.
+Qed.
+
+Lemma correct_component_derives_compliant_semantics `{MayProvide jx j} {i Ωi Ωj}
+  (c : component i jx) (ci : contract i Ωi) (cj : contract j Ωj)
+  (pred : Ωi -> Ωj -> Prop)
+  (correct : correct_component c ci cj pred)
+  (ωi : Ωi) (ωj : Ωj) (inv : pred ωi ωj)
+  (sem : semantics jx) (comp : compliant_semantics cj ωj sem)
+  : compliant_semantics ci ωi (derive_semantics c sem).
+
+Proof.
+  revert ωi ωj inv sem comp.
+  cofix correct_component_derives_compliant_semantics.
+  intros ωi ωj inv sem comp.
+  unfold correct_component in correct.
+  specialize (correct ωi ωj inv).
+  constructor; intros a e req; specialize (correct a e req);
+    destruct correct as [trust run].
+    specialize run with (eval_impure sem (c a e))
+                        (witness_impure (H := H) sem (c a e) cj ωj).
+  + apply run.
+    auto with freespec.
+  + eapply correct_component_derives_compliant_semantics.
+    ++ apply run.
+       apply respectful_impure_compliant_specs_respectful_run; auto.
+    ++ fold (exec_impure sem (c a e)).
+       auto with freespec.
+Qed.
