core/theories/Core/Interface.v
@@ -1,0 +1,380 @@
+(* FreeSpec
+ * Copyright (C) 2018–2019 ANSSI
+ *
+ * Contributors:
+ * 2018–2019 Thomas Letan <thomas.letan@ssi.gouv.fr>
+ *
+ * This impure is free software: you can redistribute it and/or modify
+ * it under the terms of the GNU General Public License as published by
+ * the Free Software Foundation, either version 3 of the License, or
+ * (at your option) any later version.
+ *
+ * This impure is distributed in the hope that it will be useful,
+ * but WITHOUT ANY WARRANTY; without even the implied warranty of
+ * MERCHANTABILITY or FITNESS FOR A PARTICULAR PURPOSE.  See the
+ * GNU General Public License for more details.
+ *
+ * You should have received a copy of the GNU General Public License
+ * along with this program. If not, see <http://www.gnu.org/licenses/>.
+ *)
+
+From Prelude Require Import All.
+From Coq Require Import Program.
+
+(** * Definition  *)
+
+(** Following the definition of the <<operational>> package, interfaces in
+    FreeSpec are parameterized inductive types whose terms purposely describe
+    the primitives the interface provides. *)
+
+Definition interface := Type -> Type.
+
+Declare Scope interface_scope.
+Bind Scope interface_scope with interface.
+
+(** Given [i : interface], a term of type [i α] identifies a primitive of [i]
+    expected to produce a result of type [α].
+
+    The simpler interface is the empty interface, which provides no primitives
+    whatsoever. *)
+
+Inductive iempty : interface := .
+
+(** Another example of general-purpose interface we can define is the [STORE s]
+    interface, where [s] is a type for a state, and [STORE s] allows for
+    manipulating a global, mutable variable of type [s] within an impure
+    computation. *)
+
+Inductive STORE (s : Type) : interface :=
+| Get : STORE s s
+| Put (x : s) : STORE s unit.
+
+Arguments Get {s}.
+Arguments Put [s] (x).
+
+(** According to the definition of [STORE s], an impure computation can use two
+    primitives. The term [Get : STORE s s] describes a primitive expected to
+    produce a result of type [s], that is the current value of the mutable
+    variable.  Terms of the form [Put x : STORE s unit] describe a primitive
+    which does not produce any meaningful result, but is expected to update the
+    current value of the mutable variable.
+
+    The use of the word “expected” to describe the primitive of [STORE s] is
+    voluntary.  The definition of an interface does not attach any particular
+    semantics to the primitives it describes.  This will come later, and in
+    fact, one interface may have many legitimate semantics.
+
+    Impure computations are likely to use more than one interface, but the
+    [impure] monad takes only one argument.  We introduce [iplus] (denoted by
+    [<+>] or [⊕]) to compose interfaces together.  An impure computation
+    parameterized by [i ⊕ j] can therefore leverage the primitives of both [i]
+    and [j]. *)
+
+(** * Interface Composites *)
+
+(** When defining general-purpose impure computations that we expect to reuse in
+    different context, we want to leave the interface as a parameter, and rather
+    express the constraints in terms of interface availability.  We tackle this
+    challenge by means of _interface composites_.
+
+    - We say an interface composite [ix] _provides_ a concrete interface [i]
+      when there exists a function [inj_p : forall α, i α -> ix α].
+    - Conversely, we can determine if a primitive of an interface composite [ix]
+      is forwarded to a concrete interface [i] when there exists a function
+      [proj_p : forall α, ix α -> option (i a)]. *)
+
+(** ** Type Classes Hierarchy *)
+
+(** We encode this mechanics using two type classes: [MayProvide], and
+    [Provide]. *)
+
+Class MayProvide (ix i : interface) : Type :=
+  { proj_p {α} (e : ix α) : option (i α)
+  }.
+
+Class Provide (ix i : interface) `{MayProvide ix i} : Type :=
+  { inj_p {α} (e : i α) : ix α
+  ; proj_inj_p_equ {α} (e : i α) : proj_p (inj_p e) = Some e
+  }.
+
+(** We provide a default instance for [MayProvide] in the form of a function
+    [proj_p] which always return [None].  We give to this default instance a
+    ridiculously high priority number to ensure it is selected only if no other
+    instances are found. *)
+
+Instance default_MayProvide (i j : interface) : MayProvide i j|1000 :=
+  { proj_p := fun _ _ => None
+  }.
+
+(** It is expected that, for an interface composite [ix] which provides [i] and
+    may provide [j], [inj_p] and [proj_p] do not mix up [i] and [j]
+    primitives. That is, injecting a primitive [e] of [i] inside [ix], then
+    projecting the resulting primitive into [j] returns [None] as long as [i]
+    and [j] are two different interfaces. *)
+
+Class Distinguish (ix i j : interface) `{Provide ix i, MayProvide ix j} : Prop :=
+  { distinguish : forall {α} (e : i α), proj_p (i := j) (inj_p (ix := ix) e) = None
+  }.
+
+(** ** Helpers *)
+
+(** Manipulating [MayProvide], [Provide] and [Distinguish] manually quickly
+    becomes verbose, especially due to the combinatorial nature of
+    [Distinguish].  In an attempt to make things easier for FreeSpec users, we
+    provide [ProvideN] and [StrictProvideN] (with [N] from [2] to
+    [5]). [ProvideN] can be used to define impure computation which use [N]
+    interfaces, while [StrictProvideN] can be used to reason about said
+    computations ([StrictProvideN] requires the [N] interfaces to be different,
+    thanks to the [Distinguish] type class). *)
+
+Class Provide2 ix i1 i2 `{Provide ix i1, Provide ix i2}.
+
+#[program]
+Instance Make_Provide2 `(Provide ix i1, Provide ix i2)
+  : Provide2 ix i1 i2.
+
+Class Provide3 ix i1 i2 i3 `{Provide ix i1, Provide ix i2, Provide ix i3}.
+
+#[program]
+Instance Make_Provide3 `(Provide ix i1, Provide ix i2, Provide ix i3)
+  : Provide3 ix i1 i2 i3.
+
+Class Provide4 ix i1 i2 i3 i4
+   `{Provide ix i1, Provide ix i2, Provide ix i3, Provide ix i4}.
+
+#[program]
+Instance Make_Provide4 `{Provide ix i1, Provide ix i2, Provide ix i3, Provide ix i4}
+  : Provide4 ix i1 i2 i3 i4.
+
+Class Provide5 ix i1 i2 i3 i4 i5
+   `{Provide ix i1, Provide ix i2, Provide ix i3, Provide ix i4, Provide ix i5}.
+
+#[program]
+Instance Make_Provide5
+   `{Provide ix i1 , Provide ix i2, Provide ix i3, Provide ix i4, Provide ix i5}
+  : Provide5 ix i1 i2 i3 i4 i5.
+
+Class StrictProvide2 ix i1 i2
+   `{Provide ix i1, Provide ix i2, ! Distinguish ix i1 i2, ! Distinguish ix i2 i1}.
+
+#[program]
+Instance Make_StrictProvide2
+   `(Provide ix i1,  Provide ix i2, ! Distinguish ix i1 i2, ! Distinguish ix i2 i1)
+  : StrictProvide2 ix i1 i2.
+
+Class StrictProvide3 (ix i1 i2 i3 : interface)
+  `{Provide ix i1, Provide ix i2, Provide ix i3, ! Distinguish ix i1 i2,
+    ! Distinguish ix i1 i3, ! Distinguish ix i2 i1, ! Distinguish ix i2 i3,
+    ! Distinguish ix i3 i1, ! Distinguish ix i3 i2}.
+
+#[program]
+Instance Make_StrictProvide3
+  `(Provide ix i1, Provide ix i2, Provide ix i3, ! Distinguish ix i1 i2,
+    ! Distinguish ix i1 i3, ! Distinguish ix i2 i1, ! Distinguish ix i2 i3,
+    ! Distinguish ix i3 i1, ! Distinguish ix i3 i2)
+  : StrictProvide3 ix i1 i2 i3.
+
+Class StrictProvide4 (ix i1 i2 i3 i4 : interface)
+  `{Provide ix i1, Provide ix i2, Provide ix i3, Provide ix i4,
+    ! Distinguish ix i1 i2, ! Distinguish ix i1 i3, ! Distinguish ix i1 i4,
+    ! Distinguish ix i2 i1, ! Distinguish ix i2 i3, ! Distinguish ix i2 i4,
+    ! Distinguish ix i3 i1, ! Distinguish ix i3 i2, ! Distinguish ix i3 i4,
+    ! Distinguish ix i4 i1, ! Distinguish ix i4 i2, ! Distinguish ix i4 i3}.
+
+#[program]
+Instance Make_StrictProvide4
+   `(Provide ix i1, Provide ix i2, Provide ix i3, Provide ix i4,
+    ! Distinguish ix i1 i2, ! Distinguish ix i1 i3, ! Distinguish ix i1 i4,
+    ! Distinguish ix i2 i1, ! Distinguish ix i2 i3, ! Distinguish ix i2 i4,
+    ! Distinguish ix i3 i1, ! Distinguish ix i3 i2, ! Distinguish ix i3 i4,
+    ! Distinguish ix i4 i1, ! Distinguish ix i4 i2, ! Distinguish ix i4 i3)
+  : StrictProvide4 ix i1 i2 i3 i4.
+
+Class StrictProvide5 (ix i1 i2 i3 i4 i5 : interface)
+   `{Provide ix i1, Provide ix i2, Provide ix i3, Provide ix i4, Provide ix i5,
+     ! Distinguish ix i1 i2, ! Distinguish ix i1 i3, ! Distinguish ix i1 i4,
+     ! Distinguish ix i1 i5, ! Distinguish ix i2 i1, ! Distinguish ix i2 i3,
+     ! Distinguish ix i2 i4, ! Distinguish ix i2 i5, ! Distinguish ix i3 i1,
+     ! Distinguish ix i3 i2, ! Distinguish ix i3 i4, ! Distinguish ix i3 i5,
+     ! Distinguish ix i4 i1, ! Distinguish ix i4 i2, ! Distinguish ix i4 i3,
+     ! Distinguish ix i4 i5, ! Distinguish ix i5 i1, ! Distinguish ix i5 i2,
+     ! Distinguish ix i5 i3, ! Distinguish ix i5 i4}.
+
+#[program]
+Instance Make_StrictProvide5 (ix i1 i2 i3 i4 i5 : interface)
+   `(Provide ix i1, Provide ix i2, Provide ix i3, Provide ix i4, Provide ix i5,
+     ! Distinguish ix i1 i2, ! Distinguish ix i1 i3, ! Distinguish ix i1 i4,
+     ! Distinguish ix i1 i5, ! Distinguish ix i2 i1, ! Distinguish ix i2 i3,
+     ! Distinguish ix i2 i4, ! Distinguish ix i2 i5, ! Distinguish ix i3 i1,
+     ! Distinguish ix i3 i2, ! Distinguish ix i3 i4, ! Distinguish ix i3 i5,
+     ! Distinguish ix i4 i1, ! Distinguish ix i4 i2, ! Distinguish ix i4 i3,
+     ! Distinguish ix i4 i5, ! Distinguish ix i5 i1, ! Distinguish ix i5 i2,
+     ! Distinguish ix i5 i3, ! Distinguish ix i5 i4)
+  : StrictProvide5 ix i1 i2 i3 i4 i5.
+
+(** ** Interfaces Sum *)
+
+(** We provide the [iplus] operator to compose interface together. That is,
+    [iplus] can be used to build _concrete_ (as opposed to polymorphic)
+    interface composite. *)
+
+Inductive iplus (i j : interface) (α : Type) :=
+| in_left (e : i α) : iplus i j α
+| in_right (e : j α) : iplus i j α.
+
+Arguments in_left [i j α] (e).
+Arguments in_right [i j α] (e).
+
+Register iplus as freespec.core.iplus.type.
+Register in_left as freespec.core.iplus.in_left.
+Register in_right as freespec.core.iplus.in_right.
+
+Infix "+" := iplus : interface_scope.
+
+(** For [iplus] to be used seamlessly as a concrete interface composite, we
+    provide the necessary instances for the [MayProvide], [Provide] and
+    [Distinguish] type classes. Note that these instances always prefer the
+    left operand of [iplus]. For instance, considering a situation where
+    there is an instace for [Provide ix i] and an instance for [Provide jx i],
+    the instance of [Provide (ix + jx) i] will rely on [ix].
+
+    The main use case for [iplus] is to locally provide an additional
+    interface. For instance, we can consider a [with_state] function which would
+    locally give access to the [STORE] interface, that is [with_state : forall
+    ix s α, s -> impure (ix + STORE s) α -> impure ix α]. In such a case, the
+    interface made locally available shall be the right operand of [iplus]. This
+    way, functions such as [with_state] are reentrant. If we take an example, the
+    following impure computation:
+
+<<
+with_state true (with_state false get)
+>>
+
+    will return false (that is, the variable in the inner store). *)
+
+Instance refl_MayProvide (i : interface) : MayProvide i i :=
+  { proj_p := fun _ e => Some e
+  }.
+
+#[program]
+Instance refl_Provide (i : interface) : @Provide i i (refl_MayProvide i) :=
+  { inj_p := fun (a : Type) (e : i a) => e
+  }.
+
+Instance iplus_left_MayProvide (ix i j : interface) `{MayProvide ix i}
+  : MayProvide (ix + j) i :=
+  { proj_p := fun _ e =>
+                match e with
+                | in_left e => proj_p e
+                | _ => None
+                end
+  }.
+
+#[program]
+Instance iplus_left_Provide (ix i j : interface) `{Provide ix i}
+  : @Provide (ix + j) i (iplus_left_MayProvide ix i j) :=
+  { inj_p := fun (a : Type) (e : i a) => in_left (inj_p e)
+  }.
+
+Next Obligation.
+  now rewrite proj_inj_p_equ.
+Qed.
+
+Instance iplus_right_MayProvide (i jx j : interface) `{MayProvide jx j}
+  : MayProvide (i + jx) j :=
+  { proj_p := fun _ e =>
+                match e with
+                | in_right e => proj_p e
+                | _ => None
+                end
+  }.
+
+#[program]
+Instance iplus_right_Provide (i jx j : interface) `{Provide jx j}
+  : @Provide (i + jx) j (iplus_right_MayProvide i jx j) :=
+  { inj_p := fun _ e => in_right (inj_p e)
+  }.
+
+Next Obligation.
+  now rewrite proj_inj_p_equ.
+Qed.
+
+(** By default, Coq inference algorithm for type classe instances inference is a
+    depth-first search. This is not without consequence in our case. For
+    instance, if we consider the search of an instance for [MayProvide (i + j)
+    j], Coq will first try [iplus_right_MayProvide] (as explained previously),
+    meaning he now search for [MayProvide i j]. It turns out such an instance
+    exists: [default_MayProvide].
+
+    To circumvent this issue, we write a dedicated tactic [find_may_provide]
+    which attempt to find an instance for [MayProvide (?ix + ?jx) ?i] with
+    [refl_MayProvide], [iplus_left_MayProvide] and [iplus_right_MayProvide]. *)
+
+Ltac find_may_provide :=
+  eapply refl_MayProvide +
+  (eapply iplus_left_MayProvide; find_may_provide) +
+  (eapply iplus_right_MayProvide; find_may_provide).
+
+Hint Extern 1 (MayProvide (iplus _ _) _) => find_may_provide : typeclass_instances.
+
+#[program]
+Instance refl_Distinguish (i j : interface)
+  : @Distinguish i i j  (@refl_MayProvide i) (@refl_Provide i) (@default_MayProvide i j).
+
+#[program]
+Instance iplus_left_default_Distinguish (ix jx i j : interface)
+   `{M1 : MayProvide ix i} `{P1 : @Provide ix i M1}
+  : @Distinguish (ix + jx) i j
+                 (@iplus_left_MayProvide ix i jx M1)
+                 (@iplus_left_Provide ix i jx M1 P1)
+                 (@default_MayProvide _ j).
+
+#[program]
+Instance iplus_right_default_Distinguish (ix jx i j : interface)
+   `{M1 : MayProvide jx i} `{P1 : @Provide jx i M1}
+  : @Distinguish (ix + jx) i j
+                 (@iplus_right_MayProvide ix jx i M1)
+                 (@iplus_right_Provide ix jx i M1 P1)
+                 (@default_MayProvide _ j).
+
+#[program]
+Instance iplus_left_may_right_Distinguish (ix jx i j : interface)
+   `{M1 : MayProvide ix i} `{P1 : @Provide ix i M1} `{M2 : MayProvide jx j}
+  : @Distinguish (ix + jx) i j
+                 (@iplus_left_MayProvide ix i jx M1)
+                 (@iplus_left_Provide ix i jx M1 P1)
+                 (@iplus_right_MayProvide ix jx j M2).
+
+#[program]
+Instance iplus_right_may_left_Distinguish (ix jx i j : interface)
+   `{M1 : MayProvide jx i} `{P1 : @Provide jx i M1} `{M2 : MayProvide ix j}
+  : @Distinguish (ix + jx) i j
+                 (@iplus_right_MayProvide ix jx i M1)
+                 (@iplus_right_Provide ix jx i M1 P1)
+                 (@iplus_left_MayProvide ix j jx M2).
+
+#[program]
+Instance iplus_left_distinguish_left_Distinguish (ix jx i j : interface)
+   `{M1 : MayProvide ix i} `{P1 : @Provide ix i M1} `{M2 : MayProvide ix j}
+   `{@Distinguish ix i j M1 P1 M2}
+  : @Distinguish (ix + jx) i j
+                 (@iplus_left_MayProvide ix i jx M1)
+                 (@iplus_left_Provide ix i jx M1 P1)
+                 (@iplus_left_MayProvide ix j jx M2).
+
+Next Obligation.
+  apply distinguish.
+Defined.
+
+#[program]
+Instance iplus_right_distinguish_right_Distinguish (ix jx i j : interface)
+   `{M1 : MayProvide jx i} `{P1 : @Provide jx i M1} `{M2 : MayProvide jx j}
+   `{@Distinguish jx i j M1 P1 M2}
+  : @Distinguish (ix + jx) i j
+                 (@iplus_right_MayProvide ix jx i M1)
+                 (@iplus_right_Provide ix jx i M1 P1)
+                 (@iplus_right_MayProvide ix jx j M2).
+
+Next Obligation.
+  apply distinguish.
+Defined.
