core/theories/Core/Semantics.v
@@ -1,0 +1,484 @@
+(* FreeSpec
+ * Copyright (C) 2018–2019 ANSSI
+ *
+ * Contributors:
+ * 2018–2019 Thomas Letan <thomas.letan@ssi.gouv.fr>
+ *
+ * This impure is free software: you can redistribute it and/or modify
+ * it under the terms of the GNU General Public License as published by
+ * the Free Software Foundation, either version 3 of the License, or
+ * (at your option) any later version.
+ *
+ * This impure is distributed in the hope that it will be useful,
+ * but WITHOUT ANY WARRANTY; without even the implied warranty of
+ * MERCHANTABILITY or FITNESS FOR A PARTICULAR PURPOSE.  See the
+ * GNU General Public License for more details.
+ *
+ * You should have received a copy of the GNU General Public License
+ * along with this program. If not, see <http://www.gnu.org/licenses/>.
+ *)
+
+(** In FreeSpec, there is no particular semantics attach to interface's
+    primitives. Once an interface has been defined, we can provide one (or
+    more) operational semantics to interpret its primitives. *)
+
+(** ** Definition *)
+
+(** An operational [semantics] for the interface [i] is coinductively defined as
+    a function which can be used to interpret any primitive of [i]; it produces
+    an [interp_out] terms. *)
+
+From Coq Require Import Program Setoid Morphisms.
+From Prelude Require Import All.
+From FreeSpec.Core Require Import Interface Impure.
+
+#[local] Open Scope signature_scope.
+
+CoInductive semantics (i : interface) : Type :=
+| mk_semantics (f : forall (α : Type), i α -> interp_out i α) : semantics i
+
+(** A term of type [interp_out i a] is therefore the result of the
+    interpretation of a given primitive [i a]. It provides a result for this
+    primitive (of type [a]), and the new semantics to use to interpret the next
+    primitive of [i]. *)
+
+with interp_out (i : interface) : Type -> Type :=
+| mk_out {α} (x : α) (sem : semantics i) : interp_out i α.
+
+Arguments mk_semantics [i] (f).
+Arguments mk_out [i α] (x sem).
+
+(** Thus, a [semantics] does not only compute a result for a primitive, but also
+    provides a new semantics.  This is necessary to model impurity: the same
+    primitive may or may not return the same result when called several
+    times. *)
+
+(** As for interfaces, the simpler [semantics] is the operational semantics for
+    [iempty], the empty interface. *)
+
+Definition iempty_semantics : semantics iempty :=
+  mk_semantics (fun α (e : iempty α) => match e with end).
+
+(** We also provide a semantics for the [STORE s] interface: *)
+
+CoFixpoint store {s} (init : s) : semantics (STORE s) :=
+  mk_semantics (fun α (e : STORE s α) =>
+                  match e with
+                  | Get => mk_out init (store init)
+                  | Put next => mk_out tt (store next)
+                  end).
+
+(** We provide several helper functions to interpret primitives with
+    semantics. *)
+
+Definition run_effect {i α} (sem : semantics i) (e : i α) : interp_out i α :=
+  match sem with mk_semantics f => f _ e end.
+
+Definition interp_result {i α} (step : interp_out i α) : α :=
+  match step with mk_out x _ => x end.
+
+Definition interp_next {i α} (step : interp_out i α) : semantics i :=
+  match step with mk_out _ sem => sem end.
+
+Definition eval_effect {i α} (sem : semantics i) (e : i α) : α :=
+  interp_result (run_effect sem e).
+
+Definition exec_effect {i α} (sem : semantics i) (e : i α) : semantics i :=
+  interp_next (run_effect sem e).
+
+(** Besides, and similarly to interfaces, operational semantics can and should
+    be composed together.  To that end, we provide the [semplus] operator. *)
+
+CoFixpoint semplus {i j} (sem_i : semantics i) (sem_j : semantics j)
+  : semantics (i + j) :=
+  mk_semantics (fun _ e =>
+                  match e with
+                  | in_left e =>
+                    let out := run_effect sem_i e in
+                    mk_out (interp_result out) (semplus (interp_next out) sem_j)
+                  | in_right e =>
+                    let out := run_effect sem_j e in
+                    mk_out (interp_result out) (semplus sem_i (interp_next out))
+                  end).
+
+Declare Scope semantics_scope.
+Bind Scope semantics_scope with semantics.
+
+Infix "*" := semplus : semantics_scope.
+
+(** ** Equivalence *)
+
+(** We say two semantics are equivalent when they produce equivalent outputs
+    given the same primitive. *)
+
+CoInductive semantics_equiv {i} : semantics i -> semantics i -> Prop :=
+| semantics_equiv_rec
+    (sem sem' : semantics i)
+    (step_equiv : forall {a} (e : i a),
+        interp_out_equiv (run_effect sem e) (run_effect sem' e))
+  : semantics_equiv sem sem'
+
+(** Two interpretation output are said equivalent when they carry the same
+    result, and they provide equivalent semantics to use afterwards. *)
+
+with interp_out_equiv {i} : forall {a : Type}, interp_out i a -> interp_out i a -> Prop :=
+| step_equiv {a}
+    (o o' : interp_out i a)
+    (res_eq : interp_result o = interp_result o')
+    (next_equiv : semantics_equiv (interp_next o) (interp_next o'))
+  : interp_out_equiv o o'.
+
+(** We prove [semantics_equiv] is an equivalence, that is the relation is (1)
+    reflexive, (2) symmetric, and (3) transitive. *)
+
+#[program]
+Instance semantics_equiv_Equivalence (i : interface) : Equivalence (@semantics_equiv i).
+
+Obligation 1.
+  cofix semantics_equiv_refl.
+  intros sem.
+  constructor.
+  intros a e.
+  constructor; [ reflexivity |].
+  apply semantics_equiv_refl.
+Qed.
+
+Obligation 2.
+  cofix semantics_equiv_sym.
+  intros sem sem' equiv.
+  destruct equiv as [sem sem' step].
+  constructor.
+  intros a e.
+  specialize step with a e.
+  destruct step.
+  constructor.
+  + now symmetry.
+  + now apply semantics_equiv_sym.
+Qed.
+
+Obligation 3.
+  cofix semantics_equiv_trans.
+  intros sem sem' sem'' equiv equiv'.
+  destruct equiv as [sem sem' equ].
+  destruct equiv' as [sem' sem'' equ'].
+  constructor; intros a e.
+  specialize equ with a e.
+  specialize equ' with a e.
+  inversion equ; ssubst.
+  inversion equ'; ssubst.
+  constructor.
+  + now transitivity (eval_effect sem' e).
+  + eapply semantics_equiv_trans; [ apply next_equiv | apply next_equiv0 ].
+Qed.
+
+(** We use [semantics_equiv] as the [Equality] relation for [semantics]. *)
+
+#[program]
+Instance semantics_Equality (i : interface) : Equality (semantics i).
+
+#[global]
+Opaque semantics_Equality.
+
+(** We proceed similarly with [interp_out_equiv]: we first prove it is an
+    equivalence, then we use this relation as the [Equality] relation for
+    [interp_out]. *)
+
+#[program]
+Instance interp_out_Equivalence : Equivalence (@interp_out_equiv i α).
+
+Obligation 1.
+  intros [x sem].
+  constructor; reflexivity.
+Qed.
+
+Obligation 2.
+  intros o o' equ.
+  inversion equ; ssubst.
+  now constructor.
+Qed.
+
+Obligation 3.
+  intros o o' o'' equ equ'.
+  inversion equ; ssubst.
+  inversion equ'; ssubst.
+  constructor.
+  + now transitivity (interp_result o').
+  + now transitivity (interp_next o').
+Qed.
+
+#[program]
+Instance interp_out_Equality (i : interface) (α : Type) : Equality (interp_out i α).
+
+#[global]
+Opaque interp_out_Equality.
+
+(** Since [interp_out_equiv] and [semantics_equiv] are two equivalence, we can
+    use them with the [rewrite] tactics, as long as we provide valid [Proper]
+    instances.  We proceed accordingly in FreeSpec.Core, as systematically as
+    possible. *)
+
+#[program]
+Instance mk_out_Proper : Proper (eq ==> 'equal ==> 'equal) (@mk_out i α).
+
+Next Obligation.
+  add_morphism_tactic.
+  intros x sem sem' equ.
+  constructor.
+  + reflexivity.
+  + apply equ.
+Qed.
+
+#[program]
+Instance run_effect_Proper : Proper ('equal ==> eq ==> 'equal) (@run_effect i α).
+
+Next Obligation.
+  add_morphism_tactic.
+  intros sem sem' equ p.
+  inversion equ; ssubst.
+  apply step_equiv0.
+Qed.
+
+#[program]
+Instance interp_result_Proper : Proper ('equal ==> eq) (@interp_result i α).
+
+Next Obligation.
+  add_morphism_tactic.
+  intros o o' equ.
+  now inversion equ; ssubst.
+Qed.
+
+#[program]
+Instance interp_next_Proper : Proper ('equal ==> 'equal) (@interp_next i α).
+
+Next Obligation.
+  add_morphism_tactic.
+  intros o o' equ.
+  now inversion equ; ssubst.
+Qed.
+
+#[program]
+Instance eval_effect_Proper : Proper ('equal ==> eq ==> eq) (@eval_effect i α).
+
+Next Obligation.
+  add_morphism_tactic.
+  intros o o' equ e.
+  unfold eval_effect.
+  now rewrite equ.
+Qed.
+
+#[program]
+Instance exec_effect_Proper : Proper ('equal ==> eq ==> 'equal) (@exec_effect i α).
+
+Next Obligation.
+  add_morphism_tactic.
+  intros o o' equ e.
+  unfold exec_effect.
+  now rewrite equ.
+Qed.
+
+Lemma semantics_equiv_interp_next_effect {i α}
+  (sem sem' : semantics i) (equ : sem == sem') (e : i α)
+  : interp_next (run_effect sem e) == interp_next (run_effect sem' e).
+
+Proof.
+  inversion equ; ssubst.
+  specialize step_equiv0 with α e.
+  inversion step_equiv0; ssubst.
+  apply next_equiv.
+Qed.
+
+Hint Resolve semantics_equiv_interp_next_effect : freespec.
+
+Lemma semantics_equiv_exec_effect {i α}
+  (sem sem' : semantics i) (equ : sem == sem') (e : i α)
+  : exec_effect sem e == exec_effect sem' e.
+
+Proof.
+  unfold exec_effect.
+  auto with freespec.
+Qed.
+
+Hint Resolve semantics_equiv_exec_effect : freespec.
+
+#[program]
+Instance semplus_Proper : Proper ('equal ==> 'equal ==> 'equal) (@semplus i j).
+
+Next Obligation.
+  add_morphism_tactic.
+  cofix semplus_Proper.
+  intros semi semi' equi semj semj' equj.
+  constructor.
+  intros a e.
+  destruct e; constructor; cbn.
+  + now rewrite equi.
+  + apply semplus_Proper; auto with freespec.
+  + now rewrite equj.
+  + apply semplus_Proper; auto with freespec.
+Qed.
+
+(** ** Interpreting Impure Computations *)
+
+(** A term of type [impure a] describes an impure computation expected to return
+    a term of type [a].  Interpreting this term means actually realizing the
+    computation and producing the result.  This requires to provide an
+    operational semantics for the interfaces used by the computation.
+
+    Some operational semantics may be defined in Gallina by means of the
+    [semantics] type. In such a case, we provide helpers functions to use them
+    in conjunction with [impure] terms. The terminology follows a similar logic than the
+    Haskell state monad:
+
+    - [run_impure] interprets an impure computation [p] with an operational
+      semantics [sem], and returns both the result of [p] and the new
+      operational semantics to use afterwards.
+    - [eval_impure] only returns the result of [p].
+    - [exec_impure] only returns the new operational semantics. *)
+
+Fixpoint run_impure {i a} (sem : semantics i) (p : impure i a) : interp_out i a :=
+  match p with
+  | local x =>
+    mk_out x sem
+  | request_then e f =>
+    let s := run_effect sem e in
+    run_impure (interp_next s) (f (interp_result s))
+  end.
+
+Definition eval_impure {i a} (sem : semantics i) (p : impure i a) : a :=
+  interp_result (run_impure sem p).
+
+Definition exec_impure {i a} (sem : semantics i) (p : impure i a) : semantics i :=
+  interp_next (run_impure sem p).
+
+(** We provide several lemmas and the necessary [Proper] instances to use these
+    functions in conjunction with [semantics_equiv] and [impure_equiv]. *)
+
+Lemma run_impure_request_then_equ {i a b} (sem : semantics i)
+  (e : i a) (f : a -> impure i b)
+  : run_impure sem (request_then e f) = run_impure (exec_effect sem e) (f (eval_effect sem e)).
+Proof eq_refl.
+
+Hint Rewrite @run_impure_request_then_equ : freespec.
+
+Lemma semantics_equiv_interp_next_impure {i a}
+  (sem sem' : semantics i) (equ : sem == sem') (p : impure i a)
+  : interp_next (run_impure sem p) == interp_next (run_impure sem' p).
+Proof.
+  revert sem sem' equ.
+  induction p; intros sem sem' equ.
+  + apply equ.
+  + cbn.
+    unfold exec_impure.
+    cbn.
+    rewrite equ at 2.
+    apply H.
+    auto with freespec.
+Qed.
+
+Hint Resolve semantics_equiv_interp_next_impure : freespec.
+
+Lemma semantics_equiv_exec_impure {i a}
+  (sem sem' : semantics i) (equ : sem == sem') (p : impure i a)
+  : exec_impure sem p == exec_impure sem' p.
+Proof.
+  unfold exec_impure.
+  auto with freespec.
+Qed.
+
+Hint Resolve semantics_equiv_exec_impure : freespec.
+
+#[program]
+Instance run_impure_Proper_1 (i : interface) (a : Type)
+  : Proper ('equal ==> eq ==> 'equal) (@run_impure i a).
+
+Next Obligation.
+  add_morphism_tactic.
+  intros sem sem' equ p.
+  revert sem sem' equ.
+  induction p; intros sem sem' equ.
+  + cbn.
+    now rewrite equ.
+  + cbn.
+    rewrite equ at 2.
+    auto with freespec.
+Qed.
+
+#[program]
+Instance run_impure_Proper_2 (i : interface) (a : Type)
+  : Proper (eq ==> 'equal ==> 'equal) (@run_impure i a).
+
+Next Obligation.
+  add_morphism_tactic.
+  intros sem p q equ.
+  revert sem.
+  induction equ; intros sem.
+  + reflexivity.
+  + apply H.
+Qed.
+
+#[program]
+Instance eval_impure_Proper (i : interface) (a : Type)
+  : Proper ('equal ==> 'equal ==> eq) (@eval_impure i a).
+
+Next Obligation.
+  add_morphism_tactic.
+  intros sem sem' equ1 p q equ2.
+  unfold eval_impure.
+  now rewrite equ1, equ2.
+Qed.
+
+#[program]
+Instance exec_impure_Proper (i : interface) (a : Type)
+  : Proper ('equal ==> 'equal ==> 'equal) (@exec_impure i a).
+
+Next Obligation.
+  add_morphism_tactic.
+  intros sem sem' equ1 p q equ2.
+  unfold exec_impure.
+  now rewrite equ1, equ2.
+Qed.
+
+Lemma run_impure_equiv {i a} (p q : impure i a) (equ : p == q) (sem : semantics i)
+  : run_impure sem p == run_impure sem q.
+Proof.
+  now rewrite equ.
+Qed.
+
+Hint Resolve run_impure_equiv : freespec.
+
+Lemma run_impure_exec_impure_equiv {i a}
+  (sem sem' : semantics i) (p q : impure i a) (equ : run_impure sem p == run_impure sem' q)
+  : exec_impure sem p == exec_impure sem' q.
+Proof.
+  now inversion equ; ssubst.
+Qed.
+
+Hint Resolve run_impure_exec_impure_equiv : freespec.
+
+Lemma run_impure_eval_impure_equiv {i a}
+  (sem sem' : semantics i) (p q : impure i a) (equ : run_impure sem p == run_impure sem' q)
+  : eval_impure sem p = eval_impure sem' q.
+Proof.
+  now inversion equ; ssubst.
+Qed.
+
+Hint Resolve run_impure_eval_impure_equiv : freespec.
+
+Lemma exec_impure_equiv {i a} (p q : impure i a) (equ : p == q) (sem : semantics i)
+  : exec_impure sem p == exec_impure sem q.
+Proof.
+  now rewrite equ.
+Qed.
+
+Hint Resolve run_impure_equiv : freespec.
+
+Lemma impure_bind_equation {i a b}
+  (p : impure i a) (f : a -> impure i b) (sem : semantics i)
+  : run_impure sem (impure_bind p f)
+    == run_impure (exec_impure sem p) (f (eval_impure sem p)).
+Proof.
+  revert sem.
+  induction p; intros sem.
+  + reflexivity.
+  + cbn.
+    apply H.
+Qed.
