core/theories/Core/Tactics.v
@@ -1,0 +1,201 @@
+(* FreeSpec
+ * Copyright (C) 2018–2019 ANSSI
+ *
+ * Contributors:
+ * 2018–2019 Thomas Letan <thomas.letan@ssi.gouv.fr>
+ *
+ * This program is free software: you can redistribute it and/or modify
+ * it under the terms of the GNU General Public License as published by
+ * the Free Software Foundation, either version 3 of the License, or
+ * (at your option) any later version.
+ *
+ * This program is distributed in the hope that it will be useful,
+ * but WITHOUT ANY WARRANTY; without even the implied warranty of
+ * MERCHANTABILITY or FITNESS FOR A PARTICULAR PURPOSE.  See the
+ * GNU General Public License for more details.
+ *
+ * You should have received a copy of the GNU General Public License
+ * along with this program. If not, see <http://www.gnu.org/licenses/>.
+ *)
+
+From Prelude Require Import All.
+From FreeSpec.Core Require Import Contract.
+
+(** The [impure] monad is an empty shell which brings structure and only
+    that.  It is not relevant when it comes to verifying impure computations,
+    and we provide a tactic called [prove_impure] to erase it while proving a
+    given impure computation is respectful wrt. to a given contract. *)
+
+Ltac destruct_if_when :=
+  let equ_cond := fresh "equ_cond" in
+  match goal with
+  | |- context[when (negb ?B) _] => case_eq B; intros equ_cond; cbn
+  | |- context[when ?B _] => case_eq B; intros equ_cond; cbn
+  | |- context[if (negb ?B) then _ else _] => case_eq B; intros equ_cond; cbn
+  | |- context[if ?B then _ else _] => case_eq B; intros equ_cond; cbn
+  | _ => idtac
+  end.
+
+Ltac destruct_if_when_in hyp :=
+  let equ_cond := fresh "equ" in
+  match type of hyp with
+  | context[when (negb ?B) _] => case_eq B;
+                                 intro equ_cond;
+                                 rewrite equ_cond in hyp
+  | context[when ?B _] => case_eq B;
+                          intro equ_cond;
+                          rewrite equ_cond in hyp
+  | context[if (negb ?B) then _ else _] => case_eq B;
+                                           intro equ_cond;
+                                           rewrite equ_cond in hyp
+  | context[if ?B then _ else _] => case_eq B;
+                                    intro equ_cond;
+                                    rewrite equ_cond in hyp
+  | _ => idtac
+  end.
+
+Ltac prove_impure :=
+  repeat (cbn -[gen_caller_obligation gen_callee_obligation gen_witness_update]; destruct_if_when);
+  lazymatch goal with
+
+  | H : ?a |- ?a => exact H
+
+  | |- _ /\ _ => split; prove_impure
+  | H : _ /\ _ |- _ => destruct H; prove_impure
+  | H : True |- _ => clear H; prove_impure
+
+  | |- context[gen_witness_update _ _ _ _] =>
+    unfold gen_witness_update;
+    repeat (rewrite proj_inj_p_equ || rewrite distinguish);
+    prove_impure
+
+  | H : context[gen_witness_update _ _ _ _] |- _ =>
+    unfold gen_witness_update in H;
+    repeat (rewrite proj_inj_p_equ in H || rewrite distinguish in H);
+    prove_impure
+
+  | |- respectful_impure ?c ?w (impure_map ?f ?p) =>
+    unfold impure_map;
+    prove_impure
+
+  | |- respectful_impure ?c ?w (impure_bind (impure_bind ?p ?f) ?g) =>
+    rewrite (impure_bind_assoc p f g);
+    prove_impure
+
+  | |- respectful_impure ?c ?w (impure_bind ?p ?f) =>
+    let x := fresh "x" in
+    let w := fresh "w" in
+    let Hrun := fresh "Hrun" in
+    apply respectful_bind_respectful_run; [| intros x w Hrun;
+                                             prove_impure ]
+
+
+  | |- respectful_impure _ _ (local _) => constructor
+  | |- respectful_impure _ _ (impure_pure _) => constructor
+
+  | |- respectful_impure ?c ?w ?p =>
+    let p := (eval hnf in p) in
+    match p with
+    | request_then ?e _ =>
+      let o_caller := fresh "o_caller" in
+      assert (o_caller : gen_caller_obligation c w e); [ prove_impure
+                                                       | constructor; prove_impure
+                                                       ]
+    | _ => idtac
+    end
+  | |- context[gen_caller_obligation _ _ _] =>
+    unfold gen_caller_obligation;
+    repeat (rewrite proj_inj_p_equ || rewrite distinguish);
+    prove_impure
+  | H: context[gen_caller_obligation _ _ _] |- _ =>
+    cbn in H;
+    unfold gen_caller_obligation in H;
+    repeat (rewrite proj_inj_p_equ in H || rewrite distinguish in H);
+    prove_impure
+
+  | |- forall _, gen_callee_obligation _ _ _ _ -> _ =>
+    let x := fresh "x" in
+    let o_caller := fresh "o_caller" in
+    intros x o_caller;
+    cbn in o_caller;
+    unfold gen_callee_obligation in o_caller;
+    repeat (rewrite proj_inj_p_equ in o_caller || rewrite distinguish in o_caller);
+    prove_impure
+
+  | |- ?a => auto
+  end.
+
+Ltac simpl_gens :=
+  cbn in *;
+  repeat lazymatch goal with
+         | H : gen_caller_obligation _ _ _ /\ gen_caller_obligation _ _ _ |- _ =>
+           destruct H
+         | H : gen_callee_obligation _ _ _ _ /\ gen_callee_obligation _ _ _ _ |- _ =>
+           destruct H
+         end;
+  repeat unfold gen_caller_obligation in *;
+  repeat unfold gen_callee_obligation in *;
+  repeat unfold gen_witness_update in *;
+  repeat
+    lazymatch goal with
+    | H : context[proj_p (inj_p ?e)] |- _ =>
+      (rewrite proj_inj_p_equ in H || rewrite distinguish in H);
+      cbn in H
+    | |- context[proj_p (inj_p ?e)] =>
+      (rewrite proj_inj_p_equ || rewrite distinguish); cbn
+    end;
+  repeat
+    lazymatch goal with
+    | H : True |- _ => clear H
+    end.
+
+Ltac unroll_respectful_run_aux run :=
+  repeat (cbn -[gen_witness_update gen_caller_obligation gen_callee_obligation] in run; destruct_if_when_in run);
+  lazymatch type of run with
+
+  | respectful_run _ (impure_pure _) _ _ _ =>
+    inversion run; ssubst; clear run
+  | respectful_run _ (local _) _ _ _ =>
+    inversion run; ssubst; clear run
+
+  | respectful_run ?c (request_then ?e ?f) ?init ?final ?res =>
+    inversion run; ssubst;
+    clear run;
+    lazymatch goal with
+    | next : respectful_run c _ _ final res |- _ =>
+      unroll_respectful_run_aux next
+    | |- _ => fail "unexpected error, consider reporting the issue"
+    end
+
+  | respectful_run ?c (impure_map ?f ?p) ?init ?final ?res =>
+    unfold impure_map in run;
+    unroll_respectful_run_aux run
+
+  | respectful_run ?c (impure_bind (impure_bind ?p ?f) ?g) ?init ?final ?res =>
+    rewrite (impure_bind_assoc p f g) in run;
+    unroll_respectful_run_aux run
+
+  | respectful_run ?c (impure_bind ?p ?f) ?init ?final ?res =>
+    apply (respectful_bind_exists_respectful_run c init final p f res) in run;
+    let run1 := fresh "run" in
+    let run2 := fresh "run" in
+    destruct run as [?ω'' [?y [run1 run2]]];
+    unroll_respectful_run_aux run1; unroll_respectful_run_aux run2
+
+  | respectful_run ?c ?p ?init ?final ?res =>
+    lazymatch (eval compute -[inj_p] in p) with
+    | request_then ?e ?f =>
+      inversion run; ssubst;
+      clear run;
+      lazymatch goal with
+      | next : respectful_run c _ _ final res |- _ =>
+        unroll_respectful_run_aux next
+      | |- _ => idtac
+      end
+    | _ => idtac
+    end
+
+  | ?e => fail "cannot handle goal of the form" e
+  end.
+
+Ltac unroll_respectful_run run := unroll_respectful_run_aux run; simpl_gens.
